Reorganisation

theories/delayed.v
@@ -4,1466 +4,206 @@ From iris.algebra Require Import agree auth excl updates local_updates.
 From esop Require Import typetranslation corecalculus specification types overlap oneshot.
 From stdpp Require Import gmap set coPset.
 
-Module Delayed(AxSem: AxiomaticSemantics).
-  Module Import Axiomatics := AxSem <+ AxiomaticFacts.
-  Instance: WaitPermissions :=
-    Build_WaitPermissions axiomaticIrisG _ (@wait).
+Section Definitions.
+  Context `{allG Σ}.
+  Local Open Scope I.
 
-  Section Definitions.
-    Context `{specStateG Σ} {Hiris: wp_axiomaticIrisG Σ} `{taskDataG Σ, InitialConfiguration}.
-    Instance: axiomaticIrisG Σ := Hiris.
-    Typeclasses Transparent axiomaticIrisG.
-    Local Open Scope I.
+  Definition simulation:
+    env → expr → hexpr → gset gname → type → hexpr → conn_map → conn_map → iProp Σ
+    := simulation_body int_s_type int_s_heap.
+  
+  Definition delayed_typed Γ η e e' A τ η' :=
+    ∀ D N σ,
+      (int_i_env Γ D N σ ∗ int_i_heap η D N)
+        -∗ WP subst (of_val <$> σ) e
+        {{ xᵢ, ∃ Nᵢ' D' d', ⌜N ≡[ not_new A ]≡ Nᵢ' ∧ D' !! RET = Some d'⌝ ∧
+                            int_i_type τ d' Nᵢ'  xᵢ ∧
+                            (□simulation Γ e' η A τ η' D D') ∧
+                            int_i_heap η' D' Nᵢ' }}.
+  Record delayed_simulation U Γ (η: hexpr) e e' A (τ: type) (η': hexpr) :=
+    Delayed {
+        ds_used_names: names Γ ∪ names η ⊆ U;
+        ds_type_e: typing U Γ e η A τ η';
+        ds_type_e': typing U Γ e' η A τ η';
+        ds_sim: delayed_typed Γ η e e' A τ η'
+      }.
+End Definitions.
 
-    Definition simulation Γ e η A τ η' D M D' M': iProp Σ :=
-      ∀ N σ, existential_triple ⊤ initial_cfg
-                                (int_s_env Γ D M N σ ∗ int_s_heap η D M N)
-                                (subst (of_val <$> σ) e)
-                                (λ v, ∃ d N',
-                                    ⌜M ≡[not_new A]≡ M' ∧ N ≡[not_new A]≡ N' ∧ D' !! RET = Some d⌝ ∧
-                                    int_s_type τ d M' N' v ∗ int_s_heap η' D' M' N').
-    
-    Definition delayed_typed Γ η e e' A τ η' :=
-      ∀ D M N σ,
-        (int_i_env Γ D M N σ ∗ int_i_heap η D M N)
-          -∗ WP subst (of_val <$> σ) e
-          {{ xᵢ, ∃ Nᵢ' M' D' d', ⌜N ≡[ not_new A ]≡ Nᵢ' ∧ M ≡[ not_new A ]≡ M' ∧
-                                 D' !! RET = Some d'⌝ ∗
-                             int_i_type τ d' M' Nᵢ'  xᵢ ∗
-                             int_i_heap η' D' M' Nᵢ' ∗
-                             □simulation Γ e' η A τ η' D M D' M' }}.
-    Record delayed_simulation U Γ (η: heap) e e' A (τ: type) (η': heap) :=
-      Delayed {
-          ds_used_names: names Γ ∪ names η ⊆ U;
-          ds_type_e: typing U Γ e η A τ η';
-          ds_type_e': typing U Γ e' η A τ η';
-          ds_sim: delayed_typed Γ η e e' A τ η'
-        }.
-
-    (** Meta-theory: The binding lemma *)
-    Definition strengthen Γ x (d: val) (D D': conn_map) := <[var x:=d]>(D ~[names_env Γ]~> D').
-    
-    Lemma strengthen_env_generic
-          (int_ty: type → @int_type Σ) (ϕ: conn_map → task_map → name_map → iProp Σ)
-          (Γ: env) (τ: type) x (D D': conn_map) v d (σ: gmap string val) (M M': task_map)
-          (N N': name_map)
-          (L: gset conn_name) (disj: names_env Γ ⊥ L) (notin: var x ∉ L) O (Osub: names Γ ⊆ O)
-          (ϕ_local: Proper (overlap L ==> eq ==> eq ==> (⊣⊢)) ϕ)
-          (int_local: ∀ τ, Proper (eq ==> overlap (names τ) ==> overlap (names τ) ==> eq ==> (⊣⊢))
-                                  (int_ty τ)):
-      intΓ int_ty Γ D M N σ -∗ (⌜N ≡[O]≡ N' ∧ M ≡[O]≡ M'⌝ ∗ int_ty τ d M' N' v ∗ ϕ D' M' N') -∗
-           let D'' := strengthen Γ x d D D' in
-           intΓ int_ty (<[x:=τ]>Γ) D'' M' N' (<[x:=v]>σ) ∗ ϕ D'' M' N'.
-    Proof.
-      iIntros "intΓ [eqN [intτ ϕ]]".
-      iDestruct "eqN" as %[eqM eqN]; cbn.
-      iSplitR "ϕ".
-      { iDestruct "intΓ" as "[dom intΓ]".
-        iDestruct "dom" as %[domσ domD].
-        iSplit.
-        { iPureIntro; split.
-          { intros y; by rewrite !lookup_insert_is_Some domσ. }
-          { intros y.
-            rewrite /strengthen !lookup_insert_is_Some.
-            intros [<-|[neqxy iny]]; first auto.
-            right; split; first congruence.
-            rewrite lookup_merge_along_in; first auto.
-            rewrite elem_of_names_env; exists y; auto. }
-        }
-        iIntros (x' τ' v' d' [lookupτ [lookupv lookupd]]).
-        destruct (decide (x=x')) as [<-|neq].
-        { rewrite lookup_insert in lookupd; injection lookupd as <-.
-          rewrite lookup_insert in lookupv; injection lookupv as <-.
-          rewrite lookup_insert in lookupτ; injection lookupτ as <-.
-          iFrame.
-        } {
-          rewrite lookup_insert_ne in lookupτ; last done.
-          rewrite lookup_insert_ne in lookupd; last congruence.
-          rewrite lookup_insert_ne in lookupv; last done.
-          iSpecialize ("intΓ" $! x' τ' v' d' with "[]").
-          { iPureIntro; repeat split; auto.
-            rewrite lookup_merge_along_in in lookupd; auto.
-            rewrite elem_of_names_env.
-            exists x'; split; eauto. }
-          assert (names τ' ⊆ O).
-          { etrans; last done.
-            intros ξ inξ.
-            rewrite env_elem_of_names; eauto. }
-          iApply (int_local with "intΓ").
-          1,4: done.
-          all: eapply overlap_mono; eauto; done. }
-      }
-      enough (overlap L D' (<[var x:=d]>(D ~[names_env Γ]~> D'))) as ov.
-      { by rewrite /strengthen -ov. }
-      intros n inn.
-      rewrite lookup_insert_ne.
-      2: by intros <-.
-      rewrite lookup_merge_along_not_in; first done.
-      clear -disj inn.
-      set_solver.
-    Qed.
-
-    Lemma good_overlap A A': not_new (A ∪ A') ⊆ not_new A ∩ not_new A'.
-    Proof.
-      intro ξ.
-      rewrite /not_new elem_of_intersection !elem_of_difference !elem_of_of_gset
-              not_elem_of_union.
-      tauto.
-    Qed.
-
-    Lemma overlap_trans {X} A A' (N N' N'': gmap gname X):
-      N ≡[not_new A]≡ N' → N' ≡[not_new A']≡ N'' →
-      N ≡[not_new (A ∪ A')]≡ N''.
-    Proof.
-      intros ov1 ov2.
-      pose proof (good_overlap A A') as ov.
-      etrans.
-      all: eapply overlap_mono.
-      2,3,6,7: done.
-      2,4: eassumption.
-      all: clear -ov.
-      all: set_solver.
-    Qed.
-
-    Local Open Scope I.
-    Context {wait_Proper: ∀ t, Proper (pointwise_relation _ (⊣⊢) ==> (⊣⊢)) (wait t)}.
-    
-    Lemma existential_part (x: string) e K Γ τ₁ τ₂ η₁ η₂ η₃ A₁ A₂ (D₁ D₂ D₃: conn_map)
-          (M₁ M₂ M₃: task_map) d
-          (d_good: D₂!!RET = Some d) (Γ_names_good: names Γ ⊥ A₁)
-          (x_fresh: ∀ e', subst_ctx (<[x:=e']>∅) K = K):
-      simulation Γ e η₁ A₁ τ₁ η₂ D₁ M₁ D₂ M₂
-                 -∗ simulation (<[x:=τ₁]>Γ) (fill_ctx x K) η₂ A₂ τ₂ η₃
-                 (strengthen Γ x d D₁ D₂) M₂ D₃ M₃
-                 -∗ simulation Γ (fill_ctx e K) η₁ (A₁ ∪ A₂) τ₂ η₃ D₁ M₁ D₃ M₃.
-    Proof.
-      iIntros "sime simK".
-      iIntros (N σ p K') "#ctx [#Γ pre] step".
-      rewrite subst_fill fill_ctx_app.
-      iMod ("sime" $! N σ p (subst_ctx (of_val <$> σ) K++K')
-              with "ctx [$Γ $pre] step") as (v₁) "[post step]".
-      iDestruct "post" as (d' N') "[props [ty pre]]".
-      iDestruct "props" as %[eqM [eqN eqd]].
-      replace d' with d in * by congruence.
-      iPoseProof (strengthen_env_generic int_s_type (int_s_heap η₂) Γ τ₁ x D₁ D₂
-                                         v₁ d σ M₁ M₂ N N' (names_heap η₂))
-        as "str".
-      { intro n.
-        rewrite elem_of_names_env.
-        rewrite /names_heap elem_of_of_list elem_of_list_fmap.
-        intros [? [-> _]] [? [[=] _]]. }
-      { rewrite /names_heap elem_of_of_list elem_of_list_fmap.
-        intros [? [[=] _]]. }
-      { done. }
-      { intros D D' eqD ?? <- ?? <-; by apply int_s_heap_local. }
-      { apply int_s_type_local. }
-      iDestruct ("str" with "Γ [$ty $pre]") as "[Γ' pre]".
-      { iPureIntro.
-        assert (of_gset (names Γ) ⊆ not_new A₁).
-        { intro ξ; rewrite elem_of_of_gset /not_new elem_of_difference elem_of_of_gset.
-          clear -Γ_names_good; set_solver. }
-        split.
-        all: apply overlap_cast.
-        all: eapply overlap_mono.
-        all: done.
-      }
-      rewrite -fill_ctx_app -(subst_val v₁ (of_val <$> σ)) -subst_fill.
-      iMod ("simK" $! N' (<[x := v₁]>σ) p K' with "ctx [$Γ' $pre] [step]")
-        as (v₂) "[post step]".
-      { rewrite fmap_insert subst_insert_r; auto using val_closed.
-        rewrite (subst_fill (<[x:=of_val v₁]>∅)) x_fresh /= lookup_insert //. }
-      iDestruct "post" as (d'' N'') "[eqs post]".
-      iModIntro.
-      iExists v₂; iFrame.
-      iExists d'', N''; iFrame.
-      iDestruct "eqs" as %[eqM' [eqN' eqd']].
-      iPureIntro; repeat split; auto.
-      all: eapply overlap_trans; eauto.
-    Qed.
-
-    Lemma wp_bind_inv K E e ϕ:
-      WP fill_ctx e K @ E {{ ϕ }} ⊢ WP e @ E {{ v, WP fill_ctx (of_val v) K @ E {{ ϕ }} }}.
-    Proof.
-      revert e ϕ.
-      induction K using rev_ind; iIntros (e ϕ) "wp"; cbn.
-      { iApply (wp_wand with "wp").
-        iIntros (v); iApply wp_value'. }
-      rewrite -!fill_ctx_app /=.
-      iPoseProof (wp_bind_item_inv with "wp") as "wp".
-      iPoseProof (IHK with "wp") as "wp".
-      iApply (wp_wand with "wp").
-      iIntros (v) "wp".
-      rewrite -fill_ctx_app /=.
-      iApply wp_bind_item; done.
-    Qed.
-    
-    Lemma wp_bind K E e ϕ:
-      WP e@E {{ v, WP fill_ctx (of_val v) K @ E {{ ϕ }} }}
-         -∗ WP fill_ctx e K @ E {{ ϕ }}.
-    Proof.
-      revert e ϕ.
-      induction K using rev_ind; iIntros (e ϕ) "wp"; cbn.
-      { iApply (wp_strong_mono with "[$wp]"); first done.
-        iIntros (v); iApply wp_value_inv. }
-      rewrite -!fill_ctx_app /=.
-      iApply wp_bind_item.
-      iApply IHK.
-      iApply (wp_wand with "wp").
-      iIntros (v) "wp".
-      iApply wp_bind_item_inv.
-      rewrite -fill_ctx_app; done.
-    Qed.
-    
-    Lemma universal_part (x: string) e e' K K' Γ τ₁ τ₂ η₁ η₂ η₃ A₁ A₂
-          (Γ_names_good: names Γ ⊥ A₁)
-          (x_fresh: ∀ e', subst_ctx (<[x:=e']>∅) K = K)
-          (x_fresh': ∀ e', subst_ctx (<[x:=e']>∅) K' = K'):
-      delayed_typed Γ η₁ e e' A₁ τ₁ η₂
-                    -∗ delayed_typed (<[x:=τ₁]>Γ) η₂ (fill_ctx x K) (fill_ctx x K') A₂ τ₂ η₃
-                    -∗ delayed_typed Γ η₁ (fill_ctx e K) (fill_ctx e' K') (A₁ ∪ A₂) τ₂ η₃.
-    Proof.
-      iIntros "dele delK".
-      iIntros (D M Ni σi) "[#intΓ intη]".
-      rewrite subst_fill.
-      iApply wp_bind.
-      iSpecialize ("dele" $! D M Ni σi with "[$intΓ $intη]").
-      iApply (wp_wand with "dele [-]").
-      iIntros (v) "post".
-      iDestruct "post" as (Ni' M' D' d') "[rel [intτ [intη' #sim]]]".
-      replace (fill_ctx (of_val v) (subst_ctx (of_val <$> σi) K))
-        with (subst (of_val <$> (<[x:=v]>σi)) (fill_ctx x K)); cycle 1.
-      { rewrite fmap_insert subst_insert_r; auto using val_closed.
-        rewrite subst_fill /= lookup_insert x_fresh -(subst_val _ (of_val <$> σi)) -subst_fill.
-        rewrite subst_val //. }
-      iDestruct "rel" as %[eqN [eqM eqd]].
-      iSpecialize ("delK" $! (strengthen Γ x d' D D') M' Ni' (<[x:=v]>σi) with "[intτ intη']").
-      { iApply (strengthen_env_generic
-                  int_i_type (int_i_heap η₂)
-                  Γ τ₁ x D D' v d' σi M M' Ni Ni' (names_heap η₂)
-                  with "intΓ [intτ intη']").
-        - intro n.
-          rewrite /names_env /names_heap !elem_of_of_list !elem_of_list_fmap.
-          intros [? [-> _]] [? [[=] _]].
-        - rewrite /names_heap elem_of_of_list elem_of_list_fmap.
-          intros [? [[=] _]].
-        - done.
-        - intros D₁ D₂ eqD ?? <- ?? <-.
-          apply int_i_heap_local; auto; done.
-        - iFrame.
-          iPureIntro.
-          assert (of_gset (names Γ) ⊆ not_new A₁).
-          { intro ξ; rewrite elem_of_of_gset /not_new elem_of_difference elem_of_of_gset.
-            clear -Γ_names_good; set_solver. }
-          split; apply overlap_cast; by eapply overlap_mono.
-      }
-      iApply (wp_wand with "delK").
-      iIntros (v') "post".
-      iDestruct "post" as (Ni'' M'' D'' d'') "[pure [intτ [intη #sim']]]".
-      iDestruct "pure" as %[eqN' [eqM' eqD']].
-      iExists Ni'', M'', D'', d''; iFrame.
+Section Meta.
+  Context `{allG Σ}.
+  Local Open Scope I.
+  (** Meta-theory: The binding lemma *)
+  Definition strengthen Γ x (d: val) (D D': conn_map) := <[var x:=d]>(D ~[conn_env Γ]~> D').
+  
+  Lemma strengthen_env_generic
+        (int_ty: type → @intT_type Σ) (ϕ: conn_map → name_map → iProp Σ)
+        (Γ: env) (τ: type) x (D D': conn_map) v d (σ: gmap string val)
+        (N N': name_map)
+        (L: gset conn_name) (disj: conn_env Γ ⊥ L) (notin: var x ∉ L) O (Osub: names Γ ⊆ O)
+        (ϕ_local: Proper (overlap L ==> eq ==> (⊣⊢)) ϕ)
+        (int_local: ∀ τ, Proper (eq ==> overlap (names τ) ==> eq ==> (⊣⊢)) (int_ty τ)):
+    int_env_pre int_ty Γ D N σ -∗ (⌜N ≡[O]≡ N'⌝ ∗ int_ty τ d N' v ∗ ϕ D' N') -∗
+         let D'' := strengthen Γ x d D D' in
+         int_env_pre int_ty (<[x:=τ]>Γ) D'' N' (<[x:=v]>σ) ∗ ϕ D'' N'.
+  Proof.
+    iIntros "intΓ [eqN [intτ ϕ]]".
+    iDestruct "eqN" as %eqN; cbn.
+    iSplitR "ϕ".
+    { iDestruct "intΓ" as "[dom intΓ]".
+      iDestruct "dom" as %[domσ domD].
       iSplit.
-      { iPureIntro; repeat split; auto.
-        all: by eapply overlap_trans; eauto. }
-      iAlways.
-      iApply (existential_part with "sim sim'"); auto.
-    Qed.
-
-    Lemma delayed_bind
-          (x: string) e e' K K' Γ τ₁ τ₂ η₁ η₂ η₃ U A₁ A₂
-          (x_fresh: ∀ e', subst_ctx (<[x:=e']>∅) K = K)
-          (x_fresh': ∀ e', subst_ctx (<[x:=e']>∅) K' = K')
-          (dele: delayed_simulation U Γ η₁ e e' A₁ τ₁ η₂)
-          (delK: delayed_simulation (U ∪ A₁) (<[x:=τ₁]>Γ) η₂ (fill_ctx x K) (fill_ctx x K') A₂ τ₂ η₃):
-      delayed_typed Γ η₁ (fill_ctx e K) (fill_ctx e' K') (A₁ ∪ A₂) τ₂ η₃.
-    Proof.
-      destruct dele as [namese tye tye' dele].
-      destruct delK as [namesK tyK tyK' delK].
-      iApply universal_part.
-      2,3: done.
-      2: iApply dele.
-      2: iApply delK.
-      apply typing_good_names in tye.
-      - destruct tye as [disj _].
-        clear -disj namese.
-        set_solver.
-      - intros x' τ' mt ξ inξ.
-        apply namese, elem_of_union, or_introl, env_elem_of_names.
-        eauto.
-      - clear -namese; set_solver.
-    Qed.
-
-    (** Meta theory: The framing lemma *)
-    Definition frame ηf (D D': conn_map): conn_map := D ~[names_heap ηf]~> D'.
-
-    Lemma frame_generic          
-          (int_ty: type → @int_type Σ) (int_he: heap → @int_heap Σ) τ (η ηf: heap)          
-          D D' d v (M M': task_map) (N N': name_map)
-          (novM: M ≡[names ηf]≡ M') (novN: N ≡[names ηf]≡ N')
-          (int_he_split: ∀ D'' M'' N'',
-              int_he (hstar η ηf) D'' M'' N'' ⊣⊢ int_he η D'' M'' N'' ∗ int_he ηf D'' M'' N'')
-          (int_he_local: ∀ η,
-              Proper (overlap (names_heap η) ==> overlap (names η) ==>
-                              overlap (names η) ==> (≡)) (int_he η))
-          (disj: names η ⊥ names ηf):
-      int_he ηf D M N -∗ (⌜D' !! RET = Some d⌝ ∗ int_ty τ d M' N' v ∗ int_he η D' M' N') -∗
-             (⌜frame ηf D D' !! RET = Some d⌝) ∗
-             int_ty τ d M' N' v ∗ int_he (hstar η ηf) (frame ηf D D') M' N'.
-    Proof.
-      iIntros "frame [eqd [type heap]]".
-      iFrame.
-      iSplitL "eqd".
-      { iDestruct "eqd" as %eqd.
-        iPureIntro.
-        rewrite /frame lookup_merge_along_not_in //.
-        rewrite /names_heap elem_of_of_list elem_of_list_fmap.
-        intros [? [[=] _]]. }
-      rewrite int_he_split.
-      iSplitL "heap".
-      - iApply (int_he_local with "heap").
-        2,3: done.
-        apply overlap_merge_along_r.
-        rewrite /names_heap => [n].
-        rewrite !elem_of_of_list !elem_of_list_fmap.
-        intros [ξ [-> inηf%elem_of_elements]] [? [[=<-] inη%elem_of_elements]].
-        apply (disj ξ); done.
-      - by iApply (int_he_local with "frame"); first apply overlap_merge_along_l.
-    Qed.
-
-    Lemma int_s_rec_split n η η' D M N:
-      int_s_heap_rec n (hstar η η') D M N ⊣⊢ int_s_heap_rec n η D M N ∗ int_s_heap_rec n η' D M N.
-    Proof. destruct n; done. Qed.
-    
-    Lemma int_s_heap_split η η' D M N:
-      int_s_heap (hstar η η') D M N ⊣⊢ (int_s_heap η D M N ∗ int_s_heap η' D M N).
-    Proof.
-      iSplit.
-      { iIntros "pre".
-        iDestruct "pre" as (n) "pre".
-        rewrite int_s_rec_split.
-        iDestruct "pre" as "[pre pre']".
-        iSplitL "pre"; iExists n; iFrame.
+      { iPureIntro; split.
+        { intros y; by rewrite !lookup_insert_is_Some domσ. }
+        { intros y.
+          rewrite /strengthen !lookup_insert_is_Some.
+          intros [<-|[neqxy iny]]; first auto.
+          right; split; first congruence.
+          rewrite lookup_merge_along_in; first auto.
+          rewrite elem_of_conn_env; exists y; auto. }
+      }
+      iIntros (x' τ' v' d' [lookupτ [lookupv lookupd]]).
+      destruct (decide (x=x')) as [<-|neq].
+      { rewrite lookup_insert in lookupd; injection lookupd as <-.
+        rewrite lookup_insert in lookupv; injection lookupv as <-.
+        rewrite lookup_insert in lookupτ; injection lookupτ as <-.
+        iFrame.
       } {
-        iIntros "[pre pre']".
-        iDestruct "pre" as (n) "pre".
-        iDestruct "pre'" as (n') "pre'".
-        iExists (max n n').
-        rewrite int_s_rec_split.
-        iSplitL "pre".
-        all: iApply int_s_heap_rec_mono; last iFrame.
-        all: auto with arith.
-      }
-    Qed.
-    
-    Lemma frame_existential Γ e (η: heap) A τ (η': heap) D D' D'' M M' (ηf: heap)
-          (disj': names η' ⊥ names ηf) (disj: names η ⊥ names ηf) (disj'': names ηf ⊥ A):
-      simulation Γ e η A τ η' D M D' M' -∗
-                 simulation Γ e (hstar η ηf) A τ (hstar η' ηf) (frame ηf D'' D) M
-                 (frame ηf D'' D') M'.
-    Proof.
-      iIntros "sim".
-      iIntros (N σ p K) "ctx [env pre] move".
-      rewrite int_s_heap_split.
-      iDestruct "pre" as "[pre frame]".
-      iMod ("sim" with "ctx [env pre] move") as (v) "[post move]".
-      { iSplitL "env".
-        - iApply (int_s_env_local with "env").
-          2-4: done.
-          symmetry.
-          apply overlap_merge_along_r.
-          rewrite /names_heap /names_env => [n].
-          rewrite !elem_of_of_list !elem_of_list_fmap.
-          intros [? [-> _]] [? [[=] _]].
-        - iApply (int_s_heap_local with "pre").
-          2-3: done.
-          symmetry.
-          apply overlap_merge_along_r.
-          rewrite /names_heap => [n].
-          rewrite !elem_of_of_list !elem_of_list_fmap.
-          intros [x [-> inη%elem_of_elements]] [? [[=<-] inηf%elem_of_elements]].
-          apply (disj x); auto. }
-      iDestruct "post" as (d N') "[eqs [type post]]".
-      iModIntro; iExists v; iFrame.
-      iDestruct "eqs" as %[eqM [eqN eqd]].
-      iExists d, N'.
-      assert (of_gset (names ηf) ⊆ not_new A).
-      { clear -disj''; intro.
-        rewrite /not_new elem_of_difference !elem_of_of_gset.
-        set_solver. }
-      iPoseProof (frame_generic int_s_type int_s_heap τ η' ηf D'' D' d v M M' N N'
-                    with "[frame] [$type $post]") as "post".
-      1,2: apply overlap_cast; eapply overlap_mono; eauto.
-      3,5: done.
-      - apply int_s_heap_split.
-      - intro; apply int_s_heap_local.
-      - iApply (int_s_heap_local with "frame").
-        2,3: done.
-        symmetry; apply overlap_merge_along_l.
-      - iDestruct "post" as "[% [$$]]"; auto.
-    Qed.
+        rewrite lookup_insert_ne in lookupτ; last done.
+        rewrite lookup_insert_ne in lookupd; last congruence.
+        rewrite lookup_insert_ne in lookupv; last done.
+        iSpecialize ("intΓ" $! x' τ' v' d' with "[]").
+        { iPureIntro; repeat split; auto.
+          rewrite lookup_merge_along_in in lookupd; auto.
+          rewrite elem_of_conn_env.
+          exists x'; split; eauto. }
+        assert (names τ' ⊆ O).
+        { etrans; last done.
+          intros ξ inξ.
+          rewrite elem_of_names_env; eauto. }
+        iApply (int_local with "intΓ").
+        1,3: done.
+        eapply overlap_sub; done. }
+    }
+    enough (overlap L D' (<[var x:=d]>(D ~[conn_env Γ]~> D'))) as ov.
+    { by rewrite /strengthen -ov. }
+    intros n inn.
+    rewrite lookup_insert_ne.
+    2: by intros <-.
+    rewrite lookup_merge_along_not_in; first done.
+    clear -disj inn.
+    set_solver.
+  Qed.
 
-    Lemma simulation_local Γ e η A τ η':
-      Proper (overlap (names_env Γ ∪ names_heap η) ==> (=) ==>
-                      overlap ({[RET]} ∪ names_heap η') ==> (=) ==> (⊣⊢))
-             (simulation Γ e η A τ η').
-    Proof.
-      iIntros (D D' eqD M M' <- E E' eqE L L' <-).
-      rewrite /simulation /existential_triple.
-      f_equiv; intro N.
-      f_equiv; intro σ.
-      f_equiv; intro p.
-      f_equiv; intro K.
-      do 2 f_equiv.
-      { f_equiv.
-        - apply int_s_env_local.
-          2-4: done.
-          eapply overlap_mono.
-          2-4: done.
-          apply union_subseteq_l.
-        - apply int_s_heap_local.
-          2,3: done.
-          eapply overlap_mono.
-          2-4: done.
-          apply union_subseteq_r. }
-      do 3 f_equiv; intro v.
-      do 2 f_equiv; intro d.
-      f_equiv; intro N'.
-      f_equiv.
-      { rewrite (eqE RET); first done.
-        clear; set_solver. }
-      f_equiv.
-      apply int_s_heap_local.
-      2,3: done.
-      eapply overlap_mono.
-      2-4: done.
-      clear; set_solver.
-    Qed.
-    
-    Lemma closed_frame Γ e e' (η: heap) A τ (η' ηf: heap)
-          (disj': names η' ⊥ names ηf) (disj: names η ⊥ names ηf) (disj'': names ηf ⊥ A):
-      delayed_typed Γ η e e' A τ η' -∗
-                    delayed_typed Γ (hstar η ηf) e e' A τ (hstar η' ηf).
-    Proof.
-      iIntros "del".
-      iIntros (D M N σ); cbn -[difference].
-      iIntros "[env [pre frame]]".
-      iSpecialize ("del" $! D M N σ with "[$env $pre]").
-      iApply (wp_wand with "del").
-      iIntros (v) "post".
-      iDestruct "post" as (N' M' D' d') "[eqs [type [post sim]]]".
-      iExists N', M', (frame ηf D D'), d'.
-      iFrame.
-      iDestruct "eqs" as %[eqM [eqN eqD']].
-      iSplit.
-      { iPureIntro; split; auto.
-        rewrite /frame lookup_merge_along_not_in; first done.
-        rewrite /names_heap elem_of_of_list elem_of_list_fmap.
-        intros [? [[=] _]]. }
-      iSplitR "sim".
-      { iSplitL "post".
-        - iApply (int_i_heap_local with "post").
-          2,3: done.
-          apply overlap_merge_along_r.
-          intro n.
-          rewrite !elem_of_names_heap.
-          intros [ξ [-> inηf]] [? [[=<-] inη']].
-          apply (disj' ξ); done.
-        - assert (of_gset (names ηf) ⊆ not_new A).
-          { clear -disj''; intro; rewrite elem_of_difference !elem_of_of_gset; set_solver. }
-          iApply (int_i_heap_local with "frame").
-          2,3: apply overlap_cast; eapply overlap_mono; done.
-          apply overlap_merge_along_l. }
-      iAssert (□simulation Γ e' (η ⊗ ηf) A τ (η' ⊗ ηf) (frame ηf D D) M (frame ηf D D') M')
-        with "[sim]" as "sim".
-      { iDestruct "sim" as "#sim"; iAlways; iApply (frame_existential with "sim"); auto. }
-      iDestruct "sim" as "#sim"; iAlways.
-      iApply (simulation_local with "sim").
-      2-4: done.
-      intros n _.
-      rewrite /frame merge_along_cases.
-      destruct bool_decide; done.
-    Qed.
-    
-    (** Meta-theory: Strengthening the environment. *)
-    Definition restrict_subst' {A} (e: option A) (τ: option type) :=
-      match τ with Some _ => e | None => None end.
-    Definition restrict_subst {A} (Γ: env) (σ: gmap string A) := merge restrict_subst' σ Γ.
-    Instance: ∀ A, DiagNone (@restrict_subst' A).
-    Proof. done. Qed.
-    Lemma lookup_restrict_subst_is_Some {A} (Γ: env) (σ: gmap string A) x:
-      is_Some (restrict_subst Γ σ !! x) ↔ is_Some (Γ!!x) ∧ is_Some (σ!!x).
-    Proof.
-      rewrite /restrict_subst lookup_merge.
-      enough (∀ o, is_Some (restrict_subst' (σ!!x) o) ↔ is_Some o ∧ is_Some (σ !! x))
-        as -> by done.
-      intros [τ|]; cbn.
-      - intuition eauto.
-      - rewrite -!not_eq_None_Some; tauto.
-    Qed.
-    
-    Lemma restrict_env (int_ty: type → @int_type Σ) Γ Γ' D M N σ (sub: Γ ⊆ Γ'):
-      intΓ int_ty Γ' D M N σ -∗ intΓ int_ty Γ D M N (restrict_subst Γ σ).
-    Proof.
-      rewrite /intΓ.
-      iIntros "[maps env]".
-      iDestruct "maps" as %[domσ domD].
-      iSplit.
-      { iPureIntro; split; intro.
-        - rewrite lookup_restrict_subst_is_Some.
-          split; last tauto.
-          intro inx; split; auto.
-          eapply domσ, lookup_weaken_is_Some; done.
-        - intro inx.
-          eapply domD, lookup_weaken_is_Some; done. }
-      iIntros (x τ v d) "pre".
-      iDestruct "pre" as %[eqτ [eqv eqd]].
-      iApply ("env" $! x τ v d).
-      iPureIntro.
-      repeat split; auto.
-      - by eapply lookup_weaken.
-      - by rewrite /restrict_subst lookup_merge eqτ in eqv.
-    Qed.
+  Lemma bind_existential_part (x: string) e K Γ τ₁ τ₂ η₁ η₂ η₃ A₁ A₂ (D₁ D₂ D₃: conn_map) d
+        (d_good: D₂!!RET = Some d) (Γ_names_good: names Γ ⊥ A₁)
+        (x_fresh: ∀ e', subst_ctx (<[x:=e']>∅) K = K):
+    simulation Γ e η₁ A₁ τ₁ η₂ D₁ D₂
+               -∗ simulation (<[x:=τ₁]>Γ) (fill_ctx x K) η₂ A₂ τ₂ η₃
+               (strengthen Γ x d D₁ D₂) D₃
+               -∗ simulation Γ (fill_ctx e K) η₁ (A₁ ∪ A₂) τ₂ η₃ D₁ D₃.
+  Proof.
+    iIntros "sime simK".
+    iIntros (N σ p K') "#ctx [#Γ pre] step".
+    rewrite subst_fill fill_ctx_app.
+    iMod ("sime" $! N σ p (subst_ctx (of_val <$> σ) K++K')
+          with "ctx [$Γ $pre] step") as (v₁) "[post step]".
+    iDestruct "post" as (d' N') "[props [ty pre]]".
+    iDestruct "props" as %[eqN eqd].
+    replace d' with d in * by congruence.
+    iPoseProof (strengthen_env_generic int_s_type (int_s_heap η₂) Γ τ₁ x D₁ D₂
+                                       v₁ d σ N N' (conn_heap η₂))
+      as "str".
+    { intro; rewrite elem_of_conn_env elem_of_conn_heap => [[? [? _]] [? [? _]]]; congruence. }
+    { by rewrite elem_of_conn_heap => [[? [? _]]]. }
+    { done. }
+    { intros D D' eqD ?? <-; by apply int_s_heap_local. }
+    iDestruct ("str" with "Γ [$ty $pre]") as "[Γ' pre]".
+    { iPureIntro.
+      assert (of_gset (names Γ) ⊆ not_new A₁).
+      { intro ξ.
+        rewrite elem_of_of_gset elem_of_not_new => [inξ].
+        intros []%Γ_names_good; done. }
+      apply overlap_cast, (overlap_sub (not_new A₁)); auto.
+    }
+    rewrite -fill_ctx_app -(subst_val v₁ (of_val <$> σ)) -subst_fill.
+    iMod ("simK" $! N' (<[x := v₁]>σ) p K' with "ctx [$Γ' $pre] [step]")
+      as (v₂) "[post step]".
+    { rewrite fmap_insert subst_insert_r; auto using val_closed.
+      rewrite (subst_fill (<[x:=of_val v₁]>∅)) x_fresh /= lookup_insert //. }
+    iDestruct "post" as (d'' N'') "[eqs post]".
+    iModIntro.
+    iExists v₂; iFrame.
+    iExists d'', N''; iFrame.
+    iDestruct "eqs" as %[eqN' eqd'].
+    iPureIntro; split; auto.
+    eapply overlap_trans; eauto.
+  Qed.
 
-    Lemma subst_restrict_with_type `(ty: typing U Γ e η A τ η'):
-      ∀ σ, subst (restrict_subst Γ σ) e = subst σ e.
-    Proof.
-      induction ty; intros; cbn.
-      1,2,3,6,7,8,9: congruence.
-      - by rewrite /restrict_subst lookup_merge Γx.
-      - rewrite IHty1; do 2 f_equal.
-        rewrite -(IHty2 (delete' x σ)); f_equal.
-        apply map_eq; intro y.
-        rewrite lookup_delete'_cases /restrict_subst !lookup_merge lookup_delete'_cases.
-        destruct (bool_decide_reflect (BNamed y ≠ x)) as [neqx|<-%dec_stable].
-        + rewrite /restrict_subst' /insert'.
-          destruct x; first done.
-          rewrite lookup_insert_ne; congruence.
-        + by destruct (insert' (BNamed y) τ₁ Γ !! y).
-    Qed.
-
-    Lemma restrict_env_fmap `(f: A → B) Γ m:
-      f <$> restrict_subst Γ m = restrict_subst Γ (f <$> m).
-    Proof.
-      apply map_eq; intro y.
-      rewrite /restrict_subst lookup_fmap !lookup_merge lookup_fmap /restrict_subst'.
-      match goal with |- f <$> match ?a with _ => _ end = _ => by destruct a end.
-    Qed.
-    
-    Lemma closed_strengthen U Γ Γ' e e' η A A' τ η'
-          (ty: typing U Γ e η A τ η')
-          (ty': typing U Γ e' η A τ η')
-          (subΓ: Γ ⊆ Γ') (subA: A ⊆ A'):
-      delayed_typed Γ η e e' A τ η' -∗ delayed_typed Γ' η e e' A' τ η'.
-    Proof.
-      assert (not_new A' ⊆ not_new A).
-      { intro; rewrite /not_new !elem_of_difference !elem_of_of_gset.
-        clear -subA; set_solver. }
-      iIntros "spec".
-      iIntros (D M N σ) "[env pre]".
-      iSpecialize ("spec" $! D M N (restrict_subst Γ σ) with "[env $pre]").
-      { by iApply (restrict_env with "env"). }
-      rewrite restrict_env_fmap (subst_restrict_with_type ty).
-      iApply (wp_wand with "spec").
-      iIntros (v) "post".
-      iDestruct "post" as (N' M' D' d') "[eqs [type [post sim]]]".
-      iExists N', M', D', d'; iFrame.
-      iDestruct "eqs" as %[eqN [eqm eqd]].
-      iSplit.
-      { iPureIntro; repeat split; auto.        
-        all: eapply overlap_mono; done. }
-      clear eqN N N' σ v.
-      iDestruct "sim" as "#sim"; iAlways.
-      iIntros (N σ p K) "ctx [env pre] move".
-      rewrite -(subst_restrict_with_type ty') -restrict_env_fmap.
-      iMod ("sim" $! N (restrict_subst Γ σ) p K with "ctx [env $pre] move") as (v) "[post move]".
-      { by iApply (restrict_env with "env"). }
-      iModIntro; iExists v; iFrame.
-      iDestruct "post" as (d N') "[eqs [type post]]".
-      iExists d, N'; iFrame.
-      iDestruct "eqs" as %[eqM [eqN eqD]].
-      iPureIntro; repeat split; auto.
-      all: by eapply overlap_mono.
-    Qed.
-
-    (** Closure: variables. *)
-    Lemma to_of_val v: to_val (of_val v) = Some v.
-    Proof.
-      destruct v; first done.
-      rewrite /= decide_left; done.
-    Qed.
-    
-    Lemma closed_variable (x: string) τ:
-      delayed_typed (<[x:=τ]>∅) hemp x x ∅ τ hemp.
-    Proof.
-      iIntros (D M N σ) "[[env_names env] _]".
-      iDestruct "env_names" as %[domσ domD].
-      assert (is_Some (σ !! x)) as [v val_x].
-      { apply domσ; rewrite lookup_insert; eauto. }
-      assert (is_Some (D !! var x)) as [d conn_x].
-      { apply domD; rewrite lookup_insert; eauto. }
-      rewrite /= lookup_fmap val_x /=.
-      iApply wp_value'.
-      iExists N, M, (<[RET:=d]>D), d.
-      rewrite /int_i_emp; iFrame.
-      iSplit.
-      { rewrite lookup_insert; auto. }
-      iSplitL "env".
-      { iApply ("env" $! x τ v d).
-        iPureIntro; split; auto.
-        apply lookup_insert. }
-      iSplit; auto.
-      iAlways.
-      iIntros (N' σ' p K) "ctx [[env_names env] heap] move".
-      iDestruct "env_names" as %[domσ' _].
-      assert (is_Some (σ' !! x)) as [v' val'_x].
-      { apply domσ'; rewrite lookup_insert; eauto. }
-      rewrite /= lookup_fmap val'_x /=.
-      iModIntro; iExists v'; iFrame.
-      iExists d, N'.
-      rewrite lookup_insert.
-      iSplit; auto.
-      iSplitL "env".
-      - iApply ("env" $! x τ v' d).
-        rewrite lookup_insert; auto.
-      - by iExists 0.
-    Qed.
-
-    (** Closure: constants. *)
-    Lemma closed_true: delayed_typed ∅ hemp Ctrue Ctrue ∅ tbool hemp.
-    Proof.
-      iIntros (D M N σ) "_".
-      change (Const Ctrue) with (of_val (VConst Ctrue)).
-      rewrite subst_closed_empty; last by apply val_closed.
-      iApply wp_value'.
-      iExists N, M, (<[RET:=VConst Ctrue]>D), (VConst Ctrue).
-      rewrite lookup_insert; iSplit; auto.
-      iSplit.
-      { iPureIntro; auto. }
-      iSplit; auto.
-      iAlways.
-      iIntros (N' σ' p K) "ctx _ move".
-      iModIntro.
-      iExists Ctrue.
-      rewrite subst_val; iFrame.
-      iExists Ctrue, N'.
-      rewrite lookup_insert; iSplit; auto.
-      iSplit.
-      - iPureIntro; auto.
-      - by iExists 0.
-    Qed.
-
-    Lemma closed_false: delayed_typed ∅ hemp Cfalse Cfalse ∅ tbool hemp.
-    Proof.
-      iIntros (D M N σ) "_".
-      change (Const Cfalse) with (of_val (VConst Cfalse)).
-      rewrite subst_closed_empty; last by apply val_closed.
-      iApply wp_value'.
-      iExists N, M, (<[RET:=VConst Cfalse]>D), (VConst Cfalse).
-      rewrite lookup_insert; iSplit; auto.
-      iSplit.
-      { iPureIntro; auto. }
-      iSplit; auto.
-      iAlways.
-      iIntros (N' σ' p K) "ctx _ move".
-      iModIntro.
-      iExists Cfalse.
-      rewrite subst_val; iFrame.
-      iExists Cfalse, N'.
-      rewrite lookup_insert; iSplit; auto.
-      iSplit.
-      - iPureIntro; auto.
-      - by iExists 0.
-    Qed.
-
-    Lemma closed_unit: delayed_typed ∅ hemp Cunit Cunit ∅ tunit hemp.
-    Proof.
-      iIntros (D M N σ) "_".
-      change (Const Cunit) with (of_val (VConst Cunit)).
-      rewrite subst_closed_empty; last by apply val_closed.
-      iApply wp_value'.
-      iExists N, M, (<[RET:=VConst Cunit]>D), (VConst Cunit).
-      rewrite lookup_insert; iSplit; auto.
-      iSplit.
-      { iPureIntro; auto. }
-      iSplit; auto.
-      iAlways.
-      iIntros (N' σ' p K) "ctx _ move".
-      iModIntro.
-      iExists Cunit.
-      rewrite subst_val; iFrame.
-      iExists Cunit, N'.
-      rewrite lookup_insert; iSplit; auto.
-      iSplit.
-      - iPureIntro; auto.
-      - by iExists 0.
-    Qed.
-
-    (** Closure: Memory operations *)
-    Lemma closed_alloc (x: string) (τ: type) ξ (ξ_fresh: ξ ∉ names τ):
-      delayed_typed (<[x:=τ]>∅) hemp (Alloc x) (Alloc x) {[ξ]} (tref ξ) (hpt ξ τ).
-    Proof.
-      iIntros (D M N σ) "[[env_names env] _]".
-      iDestruct "env_names" as %[domσ domD].
-      assert (is_Some (σ !! x)) as [v val_x].
-      { apply domσ; rewrite lookup_insert; eauto. }
-      assert (is_Some (D !! var x)) as [d conn_x].
-      { apply domD; rewrite lookup_insert; eauto. }
-      rewrite /= lookup_fmap val_x /=.
-      iApply (wp_wand with "[]").
-      { iApply wp_alloc.
-        apply to_of_val. }
-      iIntros (?) "post".
-      iDestruct "post" as (l) "[% mt]"; subst.
-      iExists (<[ξ:=Loc l]>N), M, (<[RET := d]>(<[name ξ := d]>D)), d.
-      iSplit.
-      { iPureIntro.
-        rewrite lookup_insert; repeat split; auto.
-        intro n.
-        rewrite /not_new elem_of_difference elem_of_of_gset not_elem_of_singleton => [[_ neqξ]].
-        rewrite lookup_insert_ne; congruence. }
-      iSplit.
-      { iPureIntro; exists l; rewrite lookup_insert; auto. }
-      iSplitL "mt env".
-      { iExists l, d, v; iFrame.
-        rewrite !lookup_insert lookup_insert_ne ?lookup_insert; last discriminate.
-        iSplit; auto.
-        iSpecialize  ("env" $! x τ v d with "[]").
-        { rewrite lookup_insert; auto. }
-        iApply (int_i_type_local with "env").
-        1,2,4: done.
-        intros ξ' inξ'.
-        apply lookup_insert_ne.
-        congruence. }
-      iAlways.
-      iIntros (N' σ' p K) "ctx [[env_names env] _] move".
-      iDestruct "env_names" as %[domσ' _].
-      assert (is_Some (σ' !! x)) as [v' val'_x].
-      { apply domσ'; rewrite lookup_insert; eauto. }
-      rewrite /= lookup_fmap val'_x /=.
-      iMod (simulate_alloc with "ctx move") as (l') "[move post]"; eauto using to_of_val.
-      iModIntro; iExists (Cloc l'); iFrame.
-      iExists d, (<[ξ:=Loc l']>N').
-      iSplit.
-      { rewrite lookup_insert; iPureIntro; repeat split; auto.
-        intros ξ'.
-        rewrite /not_new elem_of_difference elem_of_of_gset not_elem_of_singleton.
-        intros [_ neqξ].
-        rewrite lookup_insert_ne; done. }
-      iSplitR.
-      { iExists l'; rewrite lookup_insert; auto. }
-      iExists 0; cbn.
-      iExists l', d, v'; iFrame.
-      rewrite lookup_insert lookup_insert_ne ?lookup_insert; last discriminate.
-      iSplit; auto.
-      iSpecialize ("env" $! x τ v' d with "[]").
-      { rewrite lookup_insert; auto. }
-      iApply (int_s_type_local with "env").
-      1,2,4: done.
-      intros ξ' inξ'.
-      rewrite lookup_insert_ne; congruence.
-    Qed.
-
-    Implicit Types x y: string.
-
-    Lemma int_s_heap_pt ξ τ D M N:
-      int_s_heap (hpt ξ τ) D M N ⊣⊢ int_s_heap_rec 0 (hpt ξ τ) D M N.
-    Proof.
-      iSplit.
-      - iIntros "pre".
-        iDestruct "pre" as ([|n]) "pre"; auto.
-      - iIntros "pre".
-        iExists 0; done.
-    Qed.
-    
-    Lemma closed_read x ξ τ:
-      delayed_typed (<[x:=tref ξ]>∅) (hpt ξ τ) (Read x) (Read x) ∅ τ (hpt ξ τ).
-    Proof.
-      iIntros (D M N σ) "[[env_names env] pt]".
-      iDestruct "env_names" as %[domσ domD].
-      assert (is_Some (σ !! x)) as [v val_x].
-      { apply domσ; rewrite lookup_insert; eauto. }
-      assert (is_Some (D !! var x)) as [d conn_x].
-      { apply domD; rewrite lookup_insert; eauto. }
-      rewrite /= lookup_fmap val_x /=.
-      iDestruct ("env" $! x (tref ξ) v d with "[]") as %[l [ref ->]].
-      { rewrite lookup_insert; auto. }
-      iDestruct "pt" as (l' d' v') "[eqs [mt #val]]".
-      iDestruct "eqs" as %[ref' eqd].
-      rewrite ref in ref'; injection ref' as <-.
-      iApply (wp_wand with "[mt]").
-      { iApply (wp_read with "mt"). }
-      iIntros (v) "[% mt]"; subst v'.
-      iExists N, M, (<[RET:=d']>D), d'.
-      iFrame.
-      rewrite lookup_insert.
-      iSplit; auto.
-      iSplit; auto.
-      iSplitL.
-      { iExists l, d', v; iFrame; iSplit; auto.
-        rewrite lookup_insert_ne; auto. }
-      iClear "val".
-      clear v l val_x ref N domσ σ.
-      iAlways.
-      iIntros (N σ p K) "ctx [[env_names env] pt] move".
-      iDestruct "env_names" as %[domσ _].
-      assert (is_Some (σ !! x)) as [v val_x].
-      { apply domσ; rewrite lookup_insert; eauto. }
-      rewrite /= lookup_fmap val_x /=.
-      iDestruct ("env" $! x (tref ξ) v d with "[]") as "ref".
-      { rewrite lookup_insert; auto. }
-      iDestruct "ref" as %[l [ref ->]].
-      rewrite int_s_heap_pt.
-      iDestruct "pt" as (l' d'' v) "[eqs [pt #type]]".
-      iDestruct "eqs" as %[eql eqd'].
-      rewrite ref in eql; injection eql as <-.
-      rewrite eqd in eqd'; injection eqd' as <-.
-      iMod (simulate_read with "ctx move pt") as "[move pt]"; auto.
-      iModIntro.
-      iExists v; iFrame.
-      iExists d', N.
-      rewrite lookup_insert.
-      iSplit; first done.
-      iSplit; first done.
-      rewrite int_s_heap_pt.
-      iExists l, d', v; iFrame; iSplit; auto.
-      rewrite lookup_insert_ne; auto.
-    Qed.
-
-    Lemma closed_write x y ξ τ (neq: x ≠ y):
-      delayed_typed (<[x:=tref ξ]>(<[y:=τ]>∅)) (hpt ξ τ) (Write x y) (Write x y) ∅ tunit (hpt ξ τ).
-    Proof.
-      iIntros (D M N σ) "[[env_names #env] pt]".
-      iDestruct "env_names" as %[domσ domD].
-      assert (is_Some (σ !! x)) as [v val_x].
-      { apply domσ; rewrite lookup_insert; eauto. }
-      assert (is_Some (D !! var x)) as [d conn_x].
-      { apply domD; rewrite lookup_insert; eauto. }
-      rewrite /= lookup_fmap val_x /=.
-      assert (is_Some (σ !! y)) as [w val_y].
-      { apply domσ; rewrite lookup_insert_ne ?lookup_insert; eauto. }
-      assert (is_Some (D !! var y)) as [d' conn_y].
-      { apply domD; rewrite lookup_insert_ne ?lookup_insert; eauto. }
-      rewrite /= lookup_fmap val_y /=.
-      iDestruct "pt" as (l' dl v') "[eqs [mt #val]]".
-      iDestruct "eqs" as %[ref' eqd].
-      iDestruct ("env" $! x (tref ξ) v d with "[]") as %[l [ref ->]].
-      { rewrite lookup_insert; auto. }
-      rewrite ref in ref'; injection ref' as <-.
-      iPoseProof (wp_write ⊤ l (of_val w) w with "[mt]") as "wp".
-      { apply to_of_val. }
-      { iExists v'; iFrame. }
-      iApply (wp_wand with "wp").
-      iIntros (?) "[% mt]"; subst.
-      iExists N, M, (<[RET:=VConst Cunit]>(<[name ξ := d']>D)), Cunit.
-      rewrite lookup_insert.
-      iSplit; auto.
-      iSplit; auto.
-      iSplitL "mt".
-      { iExists l, d', w.
-        iFrame.
-        rewrite lookup_insert_ne ?lookup_insert; last auto.
-        iSplit; auto.
-        iApply ("env" $! y τ w d').
-        rewrite lookup_insert_ne; last done.
-        rewrite lookup_insert; auto. }
-      iClear "env".
-      iAlways.
-      iIntros (N' σ' p K) "ctx [[env_names #env] pt] move".
-      iDestruct "env_names" as %[domσ' _].
-      assert (is_Some (σ' !! x)) as [u val'_x].
-      { apply domσ'; rewrite lookup_insert; eauto. }
-      rewrite /= lookup_fmap val'_x /=.
-      assert (is_Some (σ' !! y)) as [w' val'_y].
-      { apply domσ'; rewrite lookup_insert_ne ?lookup_insert; eauto. }
-      rewrite lookup_fmap val'_y /=.
-      iDestruct ("env" $! x (tref ξ) u d with "[]") as %[l' [ref' ->]].
-      { rewrite lookup_insert; auto. }
-      rewrite int_s_heap_pt /= /int_s_pt.
-      iDestruct "pt" as (l'' d'' u') "[eqs [pt _]]".
-      iDestruct "eqs" as %[eql'' eqd''].
-      rewrite ref' in eql''; injection eql'' as <-.
-      rewrite eqd in eqd''; injection eqd'' as <-.
-      iMod (simulate_write with "ctx move [pt]") as "[move pt]".
-      1,2: eauto using to_of_val.
-      { iExists u'; iFrame. }
-      iModIntro; iExists Cunit; iFrame.
-      iExists Cunit, N'.
-      rewrite lookup_insert.
-      iSplit; auto.
-      iSplit; first done.
-      rewrite int_s_heap_pt.
-      iExists l', d', w'; iFrame.
-      rewrite lookup_insert_ne ?lookup_insert; last done.
-      iSplit; first done.
-      iApply ("env" $! y).
-      rewrite lookup_insert_ne ?lookup_insert; last done.
-      auto.
-    Qed.
-    
-    (** Closure: If *)
-    Lemma closed_if x Γ η A τ η' e₁ e₁' e₂ e₂' (x_type: Γ !! x = Some tbool):
-      delayed_typed Γ η e₁ e₁' A τ η' -∗
-                    delayed_typed Γ η e₂ e₂' A τ η' -∗
-                    delayed_typed Γ η (If x e₁ e₂) (If x e₁' e₂') A τ η'.
-    Proof.
-      iIntros "dtt dtf".
-      iIntros (D M N σ) "[#env pre]".
-      iPoseProof ("env") as "[env_names env_types]".
-      iDestruct "env_names" as %[domσ domD].
-      assert (is_Some (σ !! x)) as [v val_x].
-      { apply domσ; rewrite x_type; eauto. }
-      assert (is_Some (D !! var x)) as [d conn_x].
-      { apply domD; rewrite x_type; eauto. }
-      rewrite /= lookup_fmap val_x /=.
-      iDestruct ("env_types" $! x tbool v d with "[]") as %[[->| ->] <-]; first auto.
-      { iApply wp_if_true.
-        iSpecialize ("dtt" $! D M N σ with "[$env $pre]").
-        iApply (wp_wand with "dtt").
-        iClear "env env_types dtf".
-        iIntros (v) "post".
-        iDestruct "post" as (N' M' D' d') "[names [ty [heap #sim]]]".
-        iExists N', M', D', d'; iFrame.
-        clear N N' d' domσ σ val_x v.
-        iAlways.
-        iIntros (N σ p K) "#ctx [#env pre] move".
-        iPoseProof ("env") as "[env_names env_types]".
-        iDestruct "env_names" as %[domσ _].
-        assert (is_Some (σ !! x)) as [v val_x].
-        { apply domσ; rewrite x_type; eauto. }
-        iDestruct ("env_types" $! x tbool v Ctrue with "[]") as %[_ ->]; first auto.
-        rewrite /= lookup_fmap val_x /=.
-        iMod (simulate_if_true with "ctx move") as "move"; first auto.
-        iApply ("sim" with "ctx [$env $pre] move").
-      }{
-        iApply wp_if_false.
-        iSpecialize ("dtf" $! D M N σ with "[$env $pre]").
-        iApply (wp_wand with "dtf").
-        iClear "env env_types dtt".
-        iIntros (v) "post".
-        iDestruct "post" as (N' M' D' d') "[names [ty [heap #sim]]]".
-        iExists N', M', D', d'; iFrame.
-        clear N N' d' domσ σ val_x v.
-        iAlways.
-        iIntros (N σ p K) "#ctx [#env pre] move".
-        iPoseProof ("env") as "[env_names env_types]".
-        iDestruct "env_names" as %[domσ _].
-        assert (is_Some (σ !! x)) as [v val_x].
-        { apply domσ; rewrite x_type; eauto. }
-        iDestruct ("env_types" $! x tbool v Cfalse with "[]") as %[_ ->]; first auto.
-        rewrite /= lookup_fmap val_x /=.
-        iMod (simulate_if_false with "ctx move") as "move"; first auto.
-        iApply ("sim" with "ctx [$env $pre] move").
-      }
-    Qed.
-
-    (** Closure: Let *)
-    Lemma closed_let x y Γ η A τ τ' η' e e' (x_type: Γ !! x = Some τ) (y_fresh: Γ !! y = None):
-      delayed_typed (<[y:= τ]> Γ) η e e' A τ' η' -∗
-                    delayed_typed Γ η (Let (BNamed y) x e) (Let (BNamed y) x e') A τ' η'.
-    Proof.
-      iIntros "del".
-      iIntros (D M N σ) "[#env pre]".
-      iPoseProof ("env") as "[env_names env_types]".
-      iDestruct "env_names" as %[domσ domD].
-      assert (is_Some (σ !! x)) as [v val_x].
-      { apply domσ; rewrite x_type; eauto. }
-      assert (is_Some (D !! var x)) as [d conn_x].
-      { apply domD; rewrite x_type; eauto. }
-      rewrite /= lookup_fmap val_x /=.
-      iApply wp_app; first apply to_of_val.
-      rewrite /=.
-      rewrite subst_subst; cycle 1.
-      { intros x' e''.
-        rewrite lookup_delete_Some lookup_fmap fmap_Some => [[_ [v' [_ ->]]]].
-        apply val_closed. }
-      replace (subst_merge (<[y:=of_val v]> ∅) (delete y (of_val <$> σ)))
-        with (of_val <$> <[y:=v]>σ); cycle 1.
-      { apply map_eq; intro z.
-        rewrite /subst_merge lookup_merge /subst_merge'.
-        destruct (decide (y=z)) as [<-|neq].
-        - by rewrite lookup_delete lookup_fmap !lookup_insert.
-        - rewrite lookup_fmap !lookup_delete_ne; last done.
-          rewrite !lookup_insert_ne; auto.
-          rewrite lookup_empty lookup_fmap.
-          destruct (σ !! z) as [w|]; cbn; trivial.
-          rewrite subst_val; trivial. }
-      iSpecialize ("del" $! (<[var y := d]>D) M N (<[y:=v]> σ) with "[env pre]").
-      { iSplit; first iSplit.
-        - iPureIntro.
-          setoid_rewrite lookup_insert_is_Some.
-          split; first by setoid_rewrite domσ.
-          intros z [eqy|[??]]; subst; auto.
-          destruct (decide (var y = var z)); auto.
-        - iIntros (x' τ'' v' d' [mtτ [mtv mtd]]).
-          destruct (decide (y = x')) as [<-|neq].
-          + rewrite lookup_insert in mtd; injection mtd as <-.
-            rewrite lookup_insert in mtv; injection mtv as <-.
-            rewrite lookup_insert in mtτ; injection mtτ as <-.
-            iApply ("env_types" $! x); auto.
-          + rewrite lookup_insert_ne in mtd; last congruence.
-            rewrite lookup_insert_ne in mtv; last congruence.
-            rewrite lookup_insert_ne in mtτ; last congruence.
-            iApply ("env_types" $! x'); auto.
-        - iApply (int_i_heap_local with "pre").
-          2,3: done.
-          intro n.
-          rewrite /names_heap elem_of_of_list elem_of_list_fmap.
-          intros [ξ [-> _]].
-          apply lookup_insert_ne; done. }
-      iApply (wp_wand with "del").
-      iIntros (w) "post".
-      iDestruct "post" as (N' M' D' d') "[eqs [ty [heap #sim]]]".
-      iExists N', M', D', d'; iFrame.
-      iClear "env env_types".
-      clear v val_x N' d' w σ domσ N.
-      iAlways.
-      iIntros (N σ p K) "#ctx [#env pre] move".
-      cbn -[difference].
-      iPoseProof ("env") as "[env_names env_types]".
-      iDestruct "env_names" as %[domσ _].
-      assert (is_Some (σ !! x)) as [v val_x].
-      { apply domσ; rewrite x_type; eauto. }
-      rewrite /= lookup_fmap val_x /=.
-      iMod (simulate_app with "ctx move") as "move"; eauto using to_of_val.
-      rewrite /= subst_subst; cycle 1.
-      { intros x' e''.
-        rewrite lookup_delete_Some lookup_fmap fmap_Some => [[_ [v' [_ ->]]]].
-        apply val_closed. }
-      replace (subst_merge (<[y:=of_val v]> ∅) (delete y (of_val <$> σ)))
-        with (of_val <$> <[y:=v]>σ); cycle 1.
-      { apply map_eq; intro z.
-        rewrite /subst_merge lookup_merge /subst_merge'.
-        destruct (decide (y=z)) as [<-|neq].
-        - by rewrite lookup_delete lookup_fmap !lookup_insert.
-        - rewrite lookup_fmap !lookup_delete_ne; last done.
-          rewrite !lookup_insert_ne; auto.
-          rewrite lookup_empty lookup_fmap.
-          destruct (σ !! z) as [w|]; cbn; trivial.
-          rewrite subst_val; trivial. }
-      iSpecialize ("sim" $! N (<[y:=v]> σ) with "ctx [env pre]").
-      { iSplit; first iSplit.
-        - iPureIntro.
-          setoid_rewrite lookup_insert_is_Some.
-          split; first by setoid_rewrite domσ.
-          intros z [eqy|[??]]; subst; auto.
-          destruct (decide (var y = var z)); auto.
-        - iIntros (x' τ'' v' d' [mtτ [mtv mtd]]).
-          destruct (decide (y = x')) as [<-|neq].
-          + rewrite lookup_insert in mtd; injection mtd as <-.
-            rewrite lookup_insert in mtv; injection mtv as <-.
-            rewrite lookup_insert in mtτ; injection mtτ as <-.
-            iApply ("env_types" $! x); auto.
-          + rewrite lookup_insert_ne in mtd; last congruence.
-            rewrite lookup_insert_ne in mtv; last congruence.
-            rewrite lookup_insert_ne in mtτ; last congruence.
-            iApply ("env_types" $! x'); auto.
-        - iApply (int_s_heap_local with "pre").
-          2,3: done.
-          intro n.
-          rewrite /names_heap elem_of_of_list elem_of_list_fmap.
-          intros [ξ [-> _]].
-          apply lookup_insert_ne; done. }
-      iApply "sim"; auto.
-    Qed.
-
-    (** Closure: Async operations *)
-    Lemma delete_insert_eq {A} (ξ: gname) (a: A) (m: gmap gname A):
-      delete ξ m = delete ξ (<[ξ:=a]>m).
-    Proof.
-      apply map_eq; intro ξ'.
-      destruct (decide (ξ = ξ')) as [<-|neq].
-      - by rewrite !lookup_delete.
-      - by rewrite !lookup_delete_ne ?lookup_insert_ne.
-    Qed.
-
-    Ltac intro_equiv x := f_equiv; intro x.
-
-    Lemma closed_post (Γ: env) (η: heap) e e' A (τ: type) (η': heap) ξ
-          (ξ_fresh_Γ: ξ ∉ names Γ) (ξ_fresh_η: ξ ∉ names η) (ξ_fresh_A: ξ ∉ A)
-          (ξ_fresh_τ: ξ ∉ names τ) (ξ_fresh_η': ξ ∉ names η'):
-      delayed_typed Γ η e e' A τ η' -∗
-                    delayed_typed Γ η (Post e) (Post e') {[ξ]} (ttask ξ A τ) (hwait ξ A η').
-    Proof.
-      iIntros "del".
-      iIntros (D M N σ) "pre"; cbn [subst].
-      (* Allocate ghost state *)
-      iApply fupd_wp.
-      iMod (own_alloc (@unset conn_mapC)) as (γD) "ownD"; first done.
-      iMod (own_alloc (@unset name_mapC)) as (γN) "ownN"; first done.
-      iMod (own_alloc (@unset task_mapC)) as (γM) "ownM"; first done.
-      set (T := TaskData e' Γ η η' A D M γD γM γN).
-      iMod (own_alloc (to_agree T)) as (γ) "#ownγ"; first done.
-      iAssert (WP subst (of_val <$> σ) e {{ x,
-                                            int_i_promise_body int_s_type int_s_heap
-                                                               M N A τ
-                                                               (int_i_type τ) γ  x ∗
-                                                               int_i_wait_body γ η'
-                                                               (int_i_heap η') A
-                                                               M N }})
-        with "[ownD ownM ownN del pre]"
-        as "wp".
-      { iSpecialize ("del" with "pre").
-        iApply wp_fupd.
-        iApply (wp_wand with "del").
-        iIntros (v) "H".
-        iDestruct "H" as (N' M' D' d') "[eqs [ty [heap sim]]]".
-        iMod (own_update _ _ (agreed D') with "ownD") as "#ownD"; first apply oneshot_update.
-        iMod (own_update _ _ (agreed (M': task_mapC)) with "ownM") as "#ownM";
-          first apply oneshot_update.
-        iMod (own_update _ _ (agreed (N': name_mapC)) with "ownN") as "#ownN";
-          first apply oneshot_update.
-        iModIntro.
-        iDestruct "eqs" as %[eqN [eqM eqd]].
-        iSplitR "heap".
-        - iExists T, D', M', N'.
-          iSplit.
-          { repeat iSplit; auto. }
-          rewrite /ip_impl /ip_sim.
-          iSplitL "ty".
-          { iExists d'; iSplit; last done.
-            iPureIntro.
-            assert (of_gset (names τ ∖ A) ⊆ not_new A).
-            { clear; intro; rewrite /not_new elem_of_difference !elem_of_of_gset; set_solver. }
-            repeat split; auto.
-            all: apply overlap_cast; by eapply overlap_mono. }
-          iDestruct "sim" as "#sim"; iAlways.
-          iIntros (Ns Ns' σs eqNs _ p K) "ctx pre move".
-          iMod ("sim" with "ctx pre move") as (vs) "[post move]".
-          iModIntro; iExists vs; iFrame.
-          iDestruct "post" as (ds Ns'') "[maps [type heap]]".
-          iDestruct "maps" as %[eqM' [eqN' eqd']].
-          rewrite eqd in eqd'; injection eqd' as <-.
-          iExists d', (Ns'' ~[A]~> Ns).
-          iSplit.
-          { iPureIntro; split; last done.
-            intro ξ'.
-            rewrite /not_new elem_of_difference elem_of_of_gset => [[_ notinξ']].
-            rewrite lookup_merge_along_not_in; done. }
-          iSplitL "type".
-          + iApply (int_s_type_local with "type").
-            1,2,4: done.
-            intros ξ' inξ'.
-            destruct (decide (ξ' ∈ A)) as [case|case].
-            * by rewrite lookup_merge_along_in.
-            * rewrite lookup_merge_along_not_in; last done.
-              rewrite (eqNs ξ'); last rewrite elem_of_difference elem_of_union; auto.
-              rewrite (eqN' ξ'); first done.
-              rewrite /not_new elem_of_difference elem_of_of_gset; split; auto; clear; set_solver.
-          + iApply (int_s_heap_local with "heap").
-            1,2,4: done.
-            intros ξ' inξ'.
-            destruct (decide (ξ' ∈ A)) as [case|case].
-            * by rewrite lookup_merge_along_in.
-            * rewrite lookup_merge_along_not_in; last done.
-              rewrite (eqNs ξ'); last rewrite elem_of_difference elem_of_union; auto.
-              rewrite (eqN' ξ'); first done.
-              rewrite /not_new elem_of_difference elem_of_of_gset; split; auto; clear; set_solver.
-        - iExists T, D', N', M'; iFrame.
-          iSplit.
-          { by repeat iSplit. }
-          assert (of_gset (names η' ∖ A) ⊆ not_new A).
-          { clear; intro; rewrite /not_new elem_of_difference !elem_of_of_gset; set_solver. }
-          iPureIntro; split.
-          all: apply overlap_cast; eapply overlap_mono; eauto. }
-      iPoseProof (wp_post ⊤ with "wp") as "wp".
-      iModIntro.
-      iApply wp_fupd.
-      iApply (wp_wand with "wp").
-      iIntros (v) "H".
-      iDestruct "H" as (t) "[% wait]"; subst.
-      iPoseProof (wait_split with "wait") as "waits".
-      iPoseProof (fupd_mask_mono _ ⊤ with "waits") as "waits"; first auto.
-      iMod "waits" as "[promise wait]".      
-      iMod (inv_alloc promiseN with "promise") as "promise".
-      iAssert (int_i_type (Promise(ξ,A) τ) Cunit (<[ξ:=γ]>M) (<[ξ:=Task t]>N) (Ctid t))
-        with "[promise]" as "promise".
-      { cbn; iExists t, γ; iSplit.
-        - rewrite !lookup_insert; auto.
-        - iApply (inv_Proper with "promise").
-          apply wait_Proper; intro v.
-          rewrite /int_i_promise_body /ip_impl.
-          intro_equiv U; intro_equiv D'; intro_equiv M'; intro_equiv N'.          
-          do 8 f_equiv.
-          + apply (overlap_iff (names τ ∖ A)); first done.
-            intros ξ' inξ'.
-            rewrite -delete_insert_eq.
-            apply lookup_delete_ne.
-            clear -inξ' ξ_fresh_τ; set_solver.
-          + apply (overlap_iff (names τ ∖ A)); first done.
-            intros ξ' inξ'.
-            rewrite -delete_insert_eq.
-            apply lookup_delete_ne.
-            clear -inξ' ξ_fresh_τ; set_solver. }
-      iAssert (int_i_heap (Wait(ξ,A) η') (<[name ξ:=VConst Cunit]>(<[RET:=VConst Cunit]>∅))
-                          (<[ξ:=γ]>M) (<[ξ:=Task t]>N))
-        with "[wait]" as "wait".
-      { cbn; iExists t, γ.
-        rewrite !lookup_insert; iSplit; auto.
-        iApply (wait_Proper with "wait"); intro v.
-        rewrite /int_i_wait_body.
-        intro_equiv U; intro_equiv D'; intro_equiv N'; intro_equiv M'.
-        do 4 f_equiv.
-        - rewrite -!(symmetry_iff (overlap _) N').
-          apply (overlap_iff (names η' ∖ A)); first done.
-          intros ξ' inξ'.
-          rewrite -delete_insert_eq.
-          apply lookup_delete_ne.
-          clear -inξ' ξ_fresh_η'; set_solver.
-        - rewrite -!(symmetry_iff (overlap _) M').
-          apply (overlap_iff (names η' ∖ A)); first done.
-          intros ξ' inξ'.
-          rewrite -delete_insert_eq.
-          apply lookup_delete_ne.
-          clear -inξ' ξ_fresh_η'; set_solver. }
-      iModIntro.
-      iExists (<[ξ:=Task t]>N), (<[ξ:=γ]>M),
-        (<[name ξ:=VConst Cunit]>(<[RET:=VConst Cunit]>∅)), (VConst Cunit).
-      iFrame.
-      iSplit.
-      { rewrite lookup_insert_ne; last discriminate.
-        rewrite lookup_insert.
+  Lemma bind_universal_part (x: string) e e' K K' Γ τ₁ τ₂ η₁ η₂ η₃ A₁ A₂
+        (Γ_names_good: names Γ ⊥ A₁)
+        (x_fresh: ∀ e', subst_ctx (<[x:=e']>∅) K = K)
+        (x_fresh': ∀ e', subst_ctx (<[x:=e']>∅) K' = K'):
+    delayed_typed Γ η₁ e e' A₁ τ₁ η₂
+                  -∗ delayed_typed (<[x:=τ₁]>Γ) η₂ (fill_ctx x K) (fill_ctx x K') A₂ τ₂ η₃
+                  -∗ delayed_typed Γ η₁ (fill_ctx e K) (fill_ctx e' K') (A₁ ∪ A₂) τ₂ η₃.
+  Proof.
+    iIntros "dele delK".
+    iIntros (D Ni σi) "[#intΓ intη]".
+    rewrite subst_fill.
+    iApply wp_bind.
+    iSpecialize ("dele" $! D Ni σi with "[$intΓ $intη]").
+    iApply (wp_wand with "dele [-]").
+    iIntros (v) "post".
+    iDestruct "post" as (Ni' D' d') "[rel [intτ [#sim intη']]]".
+    replace (fill_ctx (of_val v) (subst_ctx (of_val <$> σi) K))
+    with (subst (of_val <$> (<[x:=v]>σi)) (fill_ctx x K)); cycle 1.
+    { rewrite fmap_insert subst_insert_r; auto using val_closed.
+      rewrite subst_fill /= lookup_insert x_fresh -(subst_val _ (of_val <$> σi)) -subst_fill.
+      rewrite subst_val //. }
+    iDestruct "rel" as %[eqN eqd].
+    iSpecialize ("delK" $! (strengthen Γ x d' D D') Ni' (<[x:=v]>σi) with "[intτ intη']").
+    { iApply (strengthen_env_generic
+                int_i_type (int_i_heap η₂) Γ τ₁ x D D' v d' σi Ni Ni' (conn_heap η₂)
+              with "intΓ [intτ intη']").
+      - intro n.
+        rewrite elem_of_conn_env elem_of_conn_heap => [[? [? _]] [? [? _]]]; congruence.
+      - rewrite elem_of_conn_heap => [[? [? _]]]; done.
+      - done.
+      - intros D₁ D₂ eqD ?? <-.
+        apply int_i_heap_local; auto; done.
+      - iFrame.
         iPureIntro.
-        repeat split.
-        all: intro ξ'; rewrite /not_new elem_of_difference elem_of_of_gset
-                               elem_of_singleton => [[_ notin]].
-        all: by rewrite lookup_insert_ne. }
-      clear σ N.
-      iAlways.
-      iIntros (N σ p K) "#ctx [env pre] move"; cbn -[difference].
-      iMod (simulate_post with "ctx move") as (p') "[move [move' neq]]"; auto.
-      iDestruct "pre" as (n) "pre".
-      iExists (Ctid p'); iFrame.
-      iExists (VConst Cunit), (<[ξ:=Task p']>N).
-      iModIntro.
-      iAssert (int_s_heap (Wait(ξ,A) η') (<[name ξ:=VConst Cunit]>(<[RET:=VConst Cunit]>∅))
-                          (<[ξ:=γ]>M) (<[ξ:=Task p']>N))
-        with "[pre move' env]" as "$".
-      { iExists (S n); cbn.
-        iExists p', γ, T, σ.
-        iSplit.
-        { iPureIntro; rewrite !lookup_insert; repeat split; auto.
-          intro ξ'.
-          rewrite elem_of_difference => [[inη' notinA]].
-          rewrite lookup_insert_ne //.
-          intros <-; contradiction.
-        }
-        iFrame.
-        iSplit; auto.
-        iExists N; iFrame. }
-      iDestruct "neq" as %neq.
-      iSplit.
-      { iPureIntro; repeat split.
-        - intros ξ'.
-          rewrite /not_new elem_of_difference elem_of_of_gset not_elem_of_singleton => [[_ ?]].
-          rewrite lookup_insert_ne; done.
-        - intros ξ'.
-          rewrite /not_new elem_of_difference elem_of_of_gset not_elem_of_singleton => [[_ ?]].
-          rewrite lookup_insert_ne; done.
-        - by rewrite lookup_insert_ne ?lookup_insert. }
-      iExists γ, T.
-      iSplit; auto.
-      iPureIntro.
-      exists p'.
-      rewrite !lookup_insert.
-      repeat split; auto.
-      intros ξ'.
-      rewrite elem_of_difference => [[inξ' _]].
-      rewrite lookup_insert_ne; cbn; congruence.
-    Qed.
+        assert (of_gset (names Γ) ⊆ not_new A₁).
+        { intro ξ; rewrite elem_of_of_gset elem_of_not_new; exact (Γ_names_good ξ). }
+        apply overlap_cast, (overlap_sub (not_new A₁)); auto.
+    }
+    iApply (wp_wand with "delK").
+    iIntros (v') "post".
+    iDestruct "post" as (Ni'' D'' d'') "[pure [intτ [#sim' intη]]]".
+    iDestruct "pure" as %[eqN' eqD'].
+    iExists Ni'', D'', d''; iFrame.
+    iSplit.
+    { iPureIntro; repeat split; eauto using overlap_trans. }
+    iAlways.
+    iApply (bind_existential_part with "sim sim'"); auto.
+  Qed.
 
-    Instance wait_proper: Proper (eq ==> pointwise_relation _ (⊣⊢) ==> (⊣⊢)) (wait (Σ := Σ)).
-    Proof. solve_proper. Qed.
-    
-    Lemma closed_wait x ξ A (τ: type) (η: heap) (nssep: (↑waitN: coPset) ⊥ ↑promiseN)
-          (ξ_not_in_τ: ξ ∉ names τ) (ξ_not_in_η: ξ ∉ names η):
-      delayed_typed (<[x:=ttask ξ A τ]>∅) (hwait ξ A η) (Wait x) (Wait x) A τ η.
-    Proof.
-      iIntros (D M N σ) "[[env_names env] pre]".
-      iDestruct "env_names" as %[domσ domD].
-      assert (is_Some (σ !! x)) as [v val_x].
-      { apply domσ; rewrite lookup_insert; eauto. }
-      assert (is_Some (D !! var x)) as [d conn_x].
-      { apply domD; rewrite lookup_insert; eauto. }
-      iDestruct ("env" $! x _ v d with "[]") as "#promise".
-      { rewrite lookup_insert; eauto. }
-      rewrite /= lookup_fmap val_x /=.
-      iDestruct "promise" as (t γ) "[eqs promise]".
-      iDestruct "eqs" as %[nameξ [mtξ ->]].
-      iApply fupd_wp.
-      iInv promiseN as "promisewait" "close".
-      rewrite /typetranslation.wp_wait /=.
-      iPoseProof (wait_split_later with "[promisewait]") as "split".
-      { iNext.
-        iApply (wait_proper with "promisewait"); first done.
-        iIntros (v); iSplit.
-        - iIntros "[pb _]"; iExact "pb".
-        - rewrite /int_i_promise_body.
-          iIntros "#pre".
-          iSplit; iExact "pre". }
-      iPoseProof (fupd_mask_mono _ (⊤ ∖ ↑promiseN) with "split") as "split"; first solve_ndisj.
-      iMod "split" as "[promisewait pw']".
-      iMod ("close" with "pw'") as "_".
-      iDestruct "pre" as (t' γ') "[mtξ' pre]".
-      rewrite mtξ nameξ.
-      iDestruct "mtξ'" as %[[=<-] [=<-]].
-      iPoseProof (wait_combine_later with "[$pre $promisewait]") as "wait".
-      iPoseProof (fupd_mask_mono _ ⊤ with "wait") as "wait"; first solve_ndisj.
-      iMod "wait" as "wait".
-      iModIntro.
-      iPoseProof (wp_wait with "wait") as "wp".
-      iApply (wp_wand with "wp").
-      iIntros (v) "[wb pb]".
-      rewrite /int_i_wait_body /int_i_promise_body.
-      iDestruct "wb" as (T D' N' M') "[[#eqT [#eqD [#eqN #eqM]]] [eqnames heap]]".
-      iClear "promise".
-      iDestruct "pb" as (T' D'' M'' N'') "[[eqT' [eqD' [eqN' eqM']]] [promise #sim]]".
-      iDestruct "promise" as (d') "[eqnames' type]".
-      iDestruct "eqnames" as %[eqN eqM].
-      iDestruct "eqnames'" as %[eqD [eqN' eqM']].
-      iPoseProof (own_valid_2 with "eqT eqT'") as "eqT'".
-      rewrite uPred.discrete_valid.
-      iDestruct "eqT'" as %?%agree_op_invL'; subst T'.
-      iPoseProof (own_valid_2 with "eqD eqD'") as "eqD'".
-      iPoseProof (own_valid_2 with "eqN eqN'") as "eqN'".
-      iPoseProof (own_valid_2 with "eqM eqM'") as "eqM'".
-      rewrite !uPred.discrete_valid.
-      iDestruct "eqD'" as %?%(agreed_valid D' D'')%leibniz_equiv; subst D''. 
-      iDestruct "eqN'" as %?%(agreed_valid N' N'')%leibniz_equiv; subst N''. 
-      iDestruct "eqM'" as %?%(agreed_valid M' M'')%leibniz_equiv; subst M''.
-      iExists (N' ~[A]~> N).
-      iExists (M' ~[A]~> M).
-      iExists (<[RET:=d']>D').
-      iExists d'.      
-      repeat iSplit.
-      1,2,3: iPureIntro.
-      { intros ξ' inξ'.
-        rewrite lookup_merge_along_not_in; first done.
-        rewrite /not_new elem_of_difference elem_of_of_gset in inξ' * => [[_ notinξ']]; done. }
-      { intros ξ' inξ'.
-        rewrite lookup_merge_along_not_in; first done.
-        rewrite /not_new elem_of_difference elem_of_of_gset in inξ' * => [[_ notinξ']]; done. }
-      { by rewrite lookup_insert. }
-      { iApply (int_i_type_local with "type").
-        1,4: done.
-        all: intros ξ' inξ'.
-        all: destruct (decide (ξ' ∈ A)) as [case|case].
-        1,3: by rewrite lookup_merge_along_in.
-        all: rewrite lookup_merge_along_not_in; last done.
-        - rewrite (eqM' ξ'); last by rewrite elem_of_difference.
-          rewrite lookup_delete_ne; first done.
-          intros <-; contradiction.
-        - rewrite (eqN' ξ'); last by rewrite elem_of_difference.
-          rewrite lookup_delete_ne; first done.
-          intros <-; contradiction. }
-      { iApply (int_i_heap_local with "heap").
-        { intro n; rewrite elem_of_names_heap; intros [ξ' [-> inξ']].
-          apply lookup_insert_ne; discriminate. }
-        all: intros ξ' inξ'.
-        all: destruct (decide (ξ' ∈ A)) as [case|case].
-        1,3: by rewrite lookup_merge_along_in.
-        all: rewrite lookup_merge_along_not_in; last done.
-        - rewrite -(eqM ξ'); last by rewrite elem_of_difference.
-          rewrite lookup_delete_ne; first done.
-          intros <-; contradiction.
-        - rewrite -(eqN ξ'); last by rewrite elem_of_difference.
-          rewrite lookup_delete_ne; first done.
-          intros <-; contradiction. }
-      iAlways.
-      iClear "eqN".
-      clear N N' eqN eqN' σ domσ val_x v nameξ.
-      iIntros (N σ p K) "#ctx [[env_names env] pre] move".
-      iDestruct "env_names" as %[domσ _].
-      assert (is_Some (σ !! x)) as [v val_x].
-      { apply domσ; rewrite lookup_insert; eauto. }
-      iSpecialize ("env" $! x _ v d with "[]").
-      { rewrite lookup_insert; auto. }
-      iRename "env" into "promise".
-      iDestruct "pre" as (n) "pre".
-      destruct n; cbn -[difference].
-      all: iDestruct "pre" as (t' γ' U σ') "[maps [ownU [move' wait]]]".
-      { iDestruct "wait" as (?) "[_ []]". }
-      iDestruct "wait" as (Npre) "pre".
-      iDestruct "promise" as (γ'' T'') "[agree'' promise]".
-      iDestruct "promise" as %[t'' [mtt'' [mtγ'' [-> eqMτ]]]].
-      iDestruct "maps" as %[mtt' [mtγ' [<- [<- eqMη]]]].
-      rewrite mtt' in mtt''; injection mtt'' as <-.
-      rewrite mtγ' in mtγ''; injection mtγ'' as <-.
-      rewrite mtξ in mtγ'; injection mtγ' as <-.
-      iPoseProof (own_valid_2 with "eqT ownU") as "ownU".
-      iPoseProof (own_valid_2 with "eqT agree''") as "agree''".
-      rewrite !uPred.discrete_valid.
-      iDestruct "ownU" as %?%(agreed_valid T U)%leibniz_equiv; subst U.
-      iDestruct "agree''" as %?%(agreed_valid T _)%leibniz_equiv; subst.
-      rewrite lookup_fmap val_x /=.
-      iMod (simulate_wait_schedule with "ctx move move'") as "[move move']"; first done.
-      rename T'' into T.
-      iSpecialize ("sim" $! (Npre ~[(names τ ∪ names (td_post T)) ∖ td_alloc T]~> N) Npre σ'
-                         (overlap_merge_along_l _ _ _) eq_refl).
-      iMod ("sim" $! _ [] with "ctx [pre] move'") as (v) "[post move']".
-      { iDestruct "pre" as "[$ pre]"; iExists n; iFrame. }
-      iDestruct "post" as (d'' N'') "[names [type heap]]".
-      iMod (simulate_done_schedule with "ctx move' move") as "[move' move]".
-      1,2: eauto using to_of_val.
-      iAssert (⌜t' ≠ p⌝) with "[move move']" as %neqp.
-      { iDestruct "move" as "[move _]".
-        iPoseProof (own_valid_2 with "move move'") as "valid".
-        rewrite /task_runnable /task_done -auth.auth_frag_op uPred.discrete_valid.
-        iDestruct "valid" as %valid; iPureIntro.
-        intros ->.
-        rewrite auth_valid_eq /= in valid.
-        specialize (valid p).
-        rewrite gmap.lookup_op !lookup_singleton in valid.
-        contradiction. }
-      iMod (simulate_wait_done with "ctx move move'") as "[move move']".
-      1,2: done.
-      iModIntro; iExists v; iFrame.
-      iExists d'', (N'' ~[ td_alloc T ]~> N); iFrame.
-      rewrite lookup_insert.
-      iDestruct "names" as %[eqN eqD'].
-      repeat iSplit.
-      1,2,3: iPureIntro.
-      - intro ξ'.
-        rewrite /not_new elem_of_difference elem_of_of_gset => [[_ notin]].
-        rewrite lookup_merge_along_not_in; done.
-      - intro ξ'.
-        rewrite /not_new elem_of_difference elem_of_of_gset => [[_ notin]].
-        rewrite lookup_merge_along_not_in; done.
-      - congruence.
-      - iApply (int_s_type_local with "type").
-        1,4: done.
-        + intros ξ' inξ'.
-          destruct (decide (ξ' ∈ td_alloc T)) as [case|case].
-          * by rewrite lookup_merge_along_in.
-          * rewrite lookup_merge_along_not_in; last done.
-            rewrite (eqM' ξ').
-            2: rewrite /not_new elem_of_difference; auto.
-            rewrite lookup_delete_ne; first done; congruence.
-        + intros ξ' inξ'.
-          destruct (decide (ξ' ∈ td_alloc T)) as [case|case].
-          * by rewrite lookup_merge_along_in.
-          * rewrite lookup_merge_along_not_in; last done.
-            rewrite -(eqN ξ').
-            2: rewrite /not_new elem_of_difference elem_of_of_gset; clear -case; set_solver.
-            rewrite lookup_merge_along_in.
-            shelve.
-      - iApply (int_s_heap_local with "post").
-        + intro n'.
-          rewrite elem_of_names_heap =>[[ξ' [-> inξ']]].
-          rewrite lookup_insert_ne; done.
-        + intros ξ' inξ'.
-          destruct (decide (ξ' ∈ td_alloc T)) as [case|case].
-          * by rewrite lookup_merge_along_in.
-          * rewrite lookup_merge_along_not_in; last done.
-            rewrite -(eqM''' ξ').
-            2: rewrite /not_new elem_of_difference elem_of_of_gset; clear -case; set_solver.
-            rewrite (eqM'' ξ'); first done.
-            rewrite elem_of_difference; auto.
-        + intros ξ' inξ'.
-          destruct (decide (ξ' ∈ td_alloc T)) as [case|case].
-          * by rewrite lookup_merge_along_in.
-          * rewrite lookup_merge_along_not_in; last done.
-            rewrite -(eqN''' ξ').
-            2: rewrite /not_new elem_of_difference elem_of_of_gset; clear -case; set_solver.
-            rewrite (eqN ξ'); first done.
-            rewrite elem_of_difference; auto.
-    Qed.
-    
+  Lemma delayed_bind
+        (x: string) e e' K K' Γ τ₁ τ₂ η₁ η₂ η₃ U A₁ A₂
+        (x_fresh: ∀ e', subst_ctx (<[x:=e']>∅) K = K)
+        (x_fresh': ∀ e', subst_ctx (<[x:=e']>∅) K' = K')
+        (dele: delayed_simulation U Γ η₁ e e' A₁ τ₁ η₂)
+        (delK: delayed_simulation (U ∪ A₁) (<[x:=τ₁]>Γ) η₂ (fill_ctx x K) (fill_ctx x K') A₂ τ₂ η₃):
+    delayed_typed Γ η₁ (fill_ctx e K) (fill_ctx e' K') (A₁ ∪ A₂) τ₂ η₃.
+  Proof.
+    destruct dele as [namese tye tye' dele].
+    destruct delK as [namesK tyK tyK' delK].
+    iApply bind_universal_part.
+    2,3: done.
+    2: iApply dele.
+    2: iApply delK.
+    apply typing_good_names in tye.
+    2,3: clear -namese; set_solver.
+    set_solver.
+  Qed.
+End Meta.
