theories/types.v
@@ -12,13 +12,13 @@ Inductive type :=
 | tref (ξ: lname)
 | ttask (ξ: lname) (A: lnames) (τ: type)
 with
-heap :=
+hexpr :=
 | hemp
-| hstar (η η': heap)
+| hstar (η η': hexpr)
 | hpt (ξ: lname) (τ: type)
-| hwait (ξ: lname) (A: lnames) (η: heap).
+| hwait (ξ: lname) (A: lnames) (η: hexpr).
 Bind Scope ty_scope with type.
-Bind Scope he_scope with heap.
+Bind Scope he_scope with hexpr.
 Notation Bool := tbool.
 Notation Unit := tunit.
 Notation "'Ref(' ξ ')'" := (tref ξ) (at level 30): ty_scope.
@@ -30,7 +30,7 @@ Notation "∅" := hemp: he_scope.
 (* TODO: Add function types. For now, we simply type let expressions. *)
 Instance: EqDecision type.
 Proof. solve_decision. Qed.
-Instance: EqDecision heap.
+Instance: EqDecision hexpr.
 Proof. solve_decision. Qed.
 
 Definition env := gmap string type.
@@ -40,7 +40,7 @@ Definition insert' {A} b (y: A) (m: gmap string A) :=
 Definition Let b e e' := App (Rec BAnon b e') e.
 
 (* TODO - figure out how to get a nice notation working. *)
-Inductive typing: lnames → env → expr → heap → lnames → type → heap → Prop :=
+Inductive typing: lnames → env → expr → hexpr → lnames → type → hexpr → Prop :=
 | tytrue U Γ: typing U Γ Ctrue ∅ ∅ Bool ∅
 | tyfalse U Γ: typing U Γ Ctrue ∅ ∅ Bool ∅
 | tyunit  U Γ: typing U Γ Cunit ∅ ∅ Unit ∅
@@ -81,16 +81,54 @@ Fixpoint he_names η: gset lname :=
   | hpt ξ τ => {[ ξ ]} ∪ ty_names τ
   | hwait ξ A η => {[ ξ ]} ∪ (he_names η ∖ A)
   end.
-Instance: Names heap := he_names.
+Instance: Names hexpr := he_names.
 
 Instance combine_names `{Names A, Names B}: Names (A*B) := λ p, names (p.1) ∪ names (p.2).
 Canonical Structure lnamesC := leibnizC lnames.
 Instance lnamesC_union: Union lnamesC := (∪).
 Instance lnamesC_monoid: Monoid lnamesC_union := Build_Monoid lnamesC (∪) ∅ _ _ _ _.
 
-Instance: Names env := λ Γ, [^ (∪) map] _ ↦ τ ∈ Γ, (names τ: lnamesC).
+Instance names_env: Names env := λ Γ, [^ (∪) map] _ ↦ τ ∈ Γ, (names τ: lnamesC).
+Lemma elem_of_names_env_empty ξ: ¬ξ ∈ names (∅: env).
+Proof. rewrite /names /names_env big_opM_empty elem_of_empty => [[]]. Qed.
+Lemma elem_of_names_env_insert x τ (Γ: env) ξ (x_fresh: Γ!!x = None):
+  ξ ∈ names (<[x:=τ]>Γ) ↔ ξ ∈ names τ ∨ ξ ∈ names Γ.
+Proof. rewrite /names /names_env big_opM_insert ?elem_of_union; done. Qed.
 
-Definition good_env U (Γ: env) := ∀ x τ, Γ!!x = Some τ → names τ ⊆ U.
+Lemma elem_of_names_env ξ (Γ: env): ξ ∈ names Γ ↔ ∃ x τ, Γ !! x = Some τ ∧ ξ ∈ names τ.
+Proof.
+  induction Γ as [|x τ Γ x_fresh IH] using map_ind.
+  - trans False.
+    { split; [apply elem_of_names_env_empty|done]. }
+    setoid_rewrite lookup_empty.
+    split; first done.
+    intros [? [? [[=] _]]].
+  - rewrite elem_of_names_env_insert ?IH; last done.
+    split.
+    { intros [inξ|[x' [τ' [mt inξ]]]].
+      { exists x, τ; rewrite lookup_insert; auto. }
+      exists x', τ'; rewrite lookup_insert_ne; auto.
+      intros <-; by rewrite x_fresh in mt. }
+    { intros [x' [τ' [mt inξ]]].
+      destruct (decide (x=x')) as [<-|neq].
+      { rewrite lookup_insert in mt; injection mt as <-; auto. }
+      rewrite lookup_insert_ne in mt; eauto. }
+Qed.
+
+Lemma elem_of_names_env_insert_gen x τ (Γ: env) ξ:
+  ξ ∈ names (<[x:=τ]>Γ) → ξ ∈ names τ ∨ ξ ∈ names Γ.
+Proof.
+  assert (<[x:=τ]>Γ = <[x:=τ]>(delete x Γ)) as ->.
+  { by apply map_eq; intro; rewrite insert_delete. }
+  rewrite elem_of_names_env_insert; last apply lookup_delete.
+  intros [case|case]; auto.
+  right.
+  rewrite elem_of_names_env in case * => [[x' [τ' [mtx inξ]]]].
+  rewrite elem_of_names_env.
+  exists x', τ'; split; auto.
+  rewrite lookup_delete_Some in mtx * => [[_ ?]]; done.
+Qed.
+
 Lemma lookup_insert' {A} x b y z (m: gmap string A):
   insert' b x m !! y = Some z ↔ (b = BNamed y ∧ x = z) ∨ (b ≠ BNamed y ∧ m!!y = Some z).
 Proof.
@@ -104,7 +142,7 @@ Qed.
 
 Lemma typing_good_names U Γ e η τ η' A:
   typing U Γ e η A τ η' →
-  good_env U Γ → names η ⊆ U →
+  names Γ ⊆ U → names η ⊆ U →
   A ⊥ U ∧ names τ ⊆ U ∪ A ∧ names η' ⊆ U ∪ A.
 Proof.
   induction 1; intros env_good pre_good; cbn -[union].
@@ -112,14 +150,20 @@ Proof.
   all: try (destruct IHtyping; auto; set_solver).
   - repeat split.
     1,3: set_solver.
-    rewrite right_id; apply (env_good x τ Γx).
+    rewrite right_id.
+    trans (names Γ); last done.
+    intro; rewrite elem_of_names_env; eauto.
   - destruct IHtyping1 as [disj1 [ty1 post1]]; auto.
     destruct IHtyping2 as [disj2 [ty2 post2]]; auto.
-    { intros x' τ'; rewrite lookup_insert'.
-      intros [[? <-]|[? ?%env_good]]; auto; set_solver. }
+    { destruct x; cbn.
+      - trans U; auto; apply union_subseteq_l.
+      - trans (names τ₁ ∪ names Γ).
+        + intro; rewrite elem_of_union; apply elem_of_names_env_insert_gen.
+        + apply union_least; auto.
+          trans U; auto; apply union_subseteq_l. }
     set_solver.
   - destruct IHtyping1 as [disj1 [ty1 post1]]; auto.
     destruct IHtyping2 as [disj2 [ty2 post2]]; auto.
-    { intros x' τ' ?%env_good; set_solver. }
+    { etrans; first done; apply union_subseteq_l. }
     set_solver.
 Qed.
