theories/typetranslation.v
@@ -1,14 +1,14 @@
 From iris.proofmode Require Import tactics classes.
 From iris.base_logic.lib Require Import invariants own.
-From iris.algebra Require Import updates agree big_op.
+From iris.algebra Require Import updates agree big_op gmap.
 From esop Require Import types oneshot specification corecalculus overlap.
 From stdpp Require Import gmap coPset.
 
 Variant name_entry := Loc (l: loc) | Task (t: tid).
 Definition name_map := gmap gname name_entry.
-Definition task_map := gmap gname gname.
+
 Variant conn_name := RET | name (ξ: gname) | var (x: string).
-Instance: EqDecision conn_name.
+Instance conn_name_eq_dec: EqDecision conn_name.
 Proof. solve_decision. Defined.
 Definition conn_name_encode c :=
   (match c with RET => 1 | name ξ => ξ~0 | var x => (encode x)~1 end)%positive.
@@ -22,193 +22,174 @@ Proof.
 Qed.
 
 Definition conn_map := gmap conn_name val.
-Definition int_type {Σ} := val → task_map → name_map → val → iProp Σ.
-Definition int_heap {Σ} := conn_map → task_map → name_map → iProp Σ.
 
-Definition names_heap (η: types.heap): gset conn_name := of_list (name <$> (elements (names η))).
-Lemma elem_of_names_heap (d: conn_name) η:
-  (d ∈ names_heap η ↔ ∃ ξ: gname, d = name ξ ∧ ξ ∈ names η)%type.
+Definition intT_type {Σ} := val → name_map → val → iProp Σ.
+Definition intT_heap {Σ} := conn_map → name_map → iProp Σ.
+
+Definition conn_heap (η: hexpr): gset conn_name := of_list (name <$> (elements (names η))).
+Lemma elem_of_conn_heap (d: conn_name) η:
+  (d ∈ conn_heap η ↔ ∃ ξ: gname, d = name ξ ∧ ξ ∈ names η)%type.
 Proof.
-  rewrite /names_heap elem_of_of_list elem_of_list_fmap.
+  rewrite /conn_heap elem_of_of_list elem_of_list_fmap.
   f_equiv; intro ξ. by rewrite elem_of_elements.
 Qed.
 
-Definition names_env (Γ: env): gset conn_name := of_list (var <$> fst <$> map_to_list Γ).
-Lemma elem_of_names_env n (Γ: env): n ∈ names_env Γ ↔ ∃ x, n = var x ∧ is_Some (Γ !! x).
+Definition conn_env (Γ: env): gset conn_name := of_list (var <$> fst <$> map_to_list Γ).
+Lemma elem_of_conn_env n (Γ: env): n ∈ conn_env Γ ↔ ∃ x, n = var x ∧ is_Some (Γ !! x).
 Proof.
-  rewrite /names_env elem_of_of_list -list_fmap_compose elem_of_list_fmap.
+  rewrite /conn_env elem_of_of_list -list_fmap_compose elem_of_list_fmap.
   split.
-  { intros [[x τ] [-> isin%elem_of_map_to_list]].
-    eauto.
-  } {
-    intros [x [-> [τ isin%elem_of_map_to_list]]].
-    exists (x,τ); auto.
-  }
-Qed.
-Lemma env_elem_of_names ξ (Γ: env): ξ ∈ names Γ ↔ ∃ x τ, Γ !! x = Some τ ∧ ξ ∈ names τ.
-Proof.
-  rewrite {1}/names /Names_instance_2.
-  induction Γ as [|x τ] using map_ind.
-  { rewrite big_opM_empty elem_of_empty.
-    setoid_rewrite lookup_empty.
-    firstorder. }
-  rewrite big_opM_insert; last done.
-  rewrite elem_of_union IHΓ.
-  split.
-  { intros [inξ|[x' [τ' [lookup inξ]]]].
-    - exists x, τ.
-      rewrite lookup_insert; auto.
-    - exists x', τ'.
-      rewrite lookup_insert_ne; auto.
-      intros <-.
-      rewrite H in lookup; discriminate. }
-  intros [x' [τ' [mt inξ]]].
-  destruct (decide (x=x')) as [<-|neq].
-  { rewrite lookup_insert in mt.
-    injection mt as <-; auto. }
-  rewrite lookup_insert_ne in mt; last done.
-  eauto.
+  { intros [[x τ] [-> isin%elem_of_map_to_list]]; eauto. }
+  { intros [x [-> [τ isin%elem_of_map_to_list]]]; exists (x,τ); auto. }
 Qed.
 
 Record task_data :=
   TaskData {
       td_expr: expr;
       td_env: env;
-      td_pre: types.heap;
-      td_post: types.heap;
+      td_pre: hexpr;
+      td_post: hexpr;
       td_alloc: gset gname;
       td_D_pre: conn_map;
-      td_M_pre: task_map;
       td_D_name: gname;
-      td_M_name: gname;
       td_N_name: gname;
     }.
+
 Canonical Structure task_dataC := leibnizC task_data.
 Canonical Structure conn_mapC := leibnizC conn_map.
 Canonical Structure name_mapC := leibnizC name_map.
-Canonical Structure task_mapC := leibnizC task_map.
+
 Class taskDataG Σ :=
   { td_common_inG:> inG Σ (agreeR task_dataC);
     td_connData_inG:> inG Σ (oneshotR conn_mapC);
     td_nameData_inG:> inG Σ (oneshotR name_mapC);
-    td_taskData_inG:> inG Σ (oneshotR task_mapC);
+    td_specNameData_inG :> inG Σ (gmapR tid (oneshotR name_mapC));
+    spec_name_map_name: gname
   }.
 Local Open Scope I.
 
-Definition intΓ {Σ} (iτ: type → int_type) (Γ: env) (D: conn_map) (M: task_map) (N: name_map)
-           (σ: gmap string val): iProp Σ :=
-  ⌜(∀ x: string, is_Some (Γ !! x) ↔ is_Some (σ !! x)) ∧
-   (∀ x: string, is_Some (Γ !! x) → is_Some (D !! var x))⌝ ∧
-  ∀ (x: string) τ v d, ⌜Γ !! x = Some τ ∧
-                       σ !! x = Some v ∧
-                       D !! var x = Some d⌝ → iτ τ d M N v.
+Definition int_env_doms (Γ: env) (D: conn_map) (σ: gmap string val): Prop :=
+  (∀ x: string, is_Some (Γ !! x) ↔ is_Some (σ !! x)) ∧
+  (∀ x: string, is_Some (Γ !! x) → is_Some (D !! var x)).
+Definition int_env_data (Γ: env) (D: conn_map) (σ: gmap string val) x τ v d: Prop :=
+  Γ !! x = Some τ ∧ σ !! x = Some v ∧ D !! var x = Some d.
+Definition int_env_pre {Σ} (iτ: type → intT_type) Γ D N σ: iProp Σ :=
+  ⌜int_env_doms Γ D σ⌝ ∧ ∀ x τ v d, ⌜int_env_data Γ D σ x τ v d⌝ → iτ τ d N v.
 
-Definition not_new A: coPset := ⊤ ∖ of_gset A.
-Class InitialConfiguration := initial_cfg: cfg.
-Class WaitPermissions :=
-  { wp_axiomaticIrisG: gFunctors → Set;
-    wp_axiomatic_implies_inv :> ∀ `{wp_axiomaticIrisG Σ}, invG Σ;
-    wp_wait: ∀ `{wp_axiomaticIrisG Σ}, tid → (val → iProp Σ) → iProp Σ }.
-Existing Class wp_axiomaticIrisG.
+Definition simulation_body `{specStateG Σ,invG Σ,inG Σ heapR,InitialConfiguration,SpecTaskDataG Σ}
+           (iτ: type → intT_type) (iη: hexpr → intT_heap)
+           Γ e η A τ η' D D': iProp Σ :=
+  ∀ N σ, existential_triple ⊤
+                            (int_env_pre iτ Γ D N σ ∗ iη η D N)
+                            (subst (of_val <$> σ) e)
+                            (λ v, ∃ d N',
+                                ⌜N ≡[not_new A]≡ N' ∧ D' !! RET = Some d⌝ ∧
+                                iτ τ d N' v ∗ iη η' D' N').
 
+Instance: ImplTaskDataT := task_data.
+Instance: SpecTaskDataT := name_map.
+
+Class allG Σ :=
+  { all_aigG :> axiomaticIrisG Σ;
+    all_ssG :> specStateG Σ;
+    all_tdG :> taskDataG Σ;
+    all_ic :> InitialConfiguration;
+    all_stdG :> SpecTaskDataG Σ }.
+    
 Section TypeInterpretation.
-  Context `{WaitPermissions, implStateG Σ, specStateG Σ, taskDataG Σ}.
-  Context `{wp_axiomaticIrisG _ Σ,InitialConfiguration}.
+  Context `{allG Σ}.
   Implicit Type d : val.
   Implicit Type N: name_map.
-  Implicit Type M: task_map.
   Implicit Type x: val.
 
-  Definition int_i_bool d M N x: iProp Σ := ⌜(x = Ctrue ∨ x = Cfalse) ∧ x = d⌝.
-  Definition int_s_bool := int_i_bool.
-  Definition int_i_unit d M N x: iProp Σ := ⌜x = Cunit⌝.
-  Definition int_s_unit := int_i_unit.
-  Definition int_i_ref (ξ: gname) d M N x: iProp Σ := ⌜∃ l: loc, N!!ξ = Some (Loc l) ∧ x = Cloc l⌝.
-  Definition int_s_ref := int_i_ref.
-  Definition int_s_promise ξ A (τ: type) d M N x: iProp Σ :=
-    ∃ γ (T: task_dataC),
-      own γ (to_agree T) ∗ 
-          ⌜∃ t, N!!ξ = Some (Task t) ∧ M!!ξ = Some γ ∧ x = Ctid t ∧
-                td_M_pre T ≡[names τ ∖ A]≡ M⌝.
+  Definition int_i_bool d N x: iProp Σ := ⌜(x = Ctrue ∨ x = Cfalse) ∧ x = d⌝.
+  Definition int_s_bool d N x := int_i_bool d N x.
+  Definition int_i_unit d N x: iProp Σ := ⌜x = Cunit⌝.
+  Definition int_s_unit d N x := int_i_unit d N x.
+  Definition int_i_ref (ξ: gname) d N x: iProp Σ := ⌜∃ l: loc, N!!ξ = Some (Loc l) ∧ x = Cloc l⌝.
+  Definition int_s_ref ξ d N x := int_i_ref ξ d N x.
+
+  Definition int_s_promise ξ A (τ: type) d N x: iProp Σ :=
+    ∃ t (Npre: name_mapC), spec_task_agree t Npre ∗
+          ⌜N!!ξ = Some (Task t) ∧ Npre ≡[names τ ∖ A]≡ N⌝.
+
+  (* Why is this needed? FIXME *)
+  Global Instance: implStateG Σ := aig_impl_state.
 
   (** We build the implementation interpretation of promise in stages. *)
   (** Access to the task data. *)
-  Definition ip_data γ U (D': conn_map) (M': task_map) (N': name_map) :=
-    own γ (to_agree U) ∗ own (td_D_name U) (agreed D') ∗ own (td_N_name U) (agreed N') ∗
-        own (td_M_name U) (agreed M').
+  Definition ip_data (t: tid) (U: task_dataC) (D': conn_map) (N': name_map): iProp Σ :=
+    task_agree t U ∗ own (td_D_name U) (agreed D') ∗ own (td_N_name U) (agreed N').
   
   (** The easy parts: name map and implementation interpretation. *)
-  Definition ip_impl (A: gset gname) (τ: type) (τi: @int_type Σ) (D': conn_map) M' N' M N y :=
-    ∃ d, ⌜D' !! RET = Some d ∧ N' ≡[ names τ ∖ A ]≡ N ∧ M' ≡[ names τ ∖ A]≡ M⌝ ∗ τi d M' N' y.
-  Definition ip_sim iτs iηs A (τ: type) U D' M': iProp Σ :=
-    ∀ N N' σ (eqN: N ≡[(names τ ∪ names (td_post U)) ∖ td_alloc U]≡ N') (eqA: td_alloc U = A),
-      existential_triple ⊤ initial_cfg
-                         (intΓ iτs (td_env U) (td_D_pre U) (td_M_pre U) N' σ ∗
-                               iηs (td_pre U) (td_D_pre U) (td_M_pre U) N')
-                         (subst (of_val <$> σ) (td_expr U))
-                         (λ v, ∃ d N'', ⌜N ≡[not_new (td_alloc U)]≡ N'' ∧ D' !! RET = Some d⌝ ∧
-                                        iτs τ d M' N'' v ∗ iηs (td_post U) D' M' N'').
+  Definition ip_impl (A: gset gname) (τ: type) (τi: @intT_type Σ) (D': conn_map) N' N y :=
+    ∃ d, ⌜D' !! RET = Some d ∧ N' ≡[ names τ ∖ A ]≡ N⌝ ∗ τi d N' y.
+  Definition ip_sim (iτs: type → @intT_type Σ) (iηs: hexpr → @intT_heap Σ)
+             A (τ: type) U D': iProp Σ :=
+    ⌜A = td_alloc U⌝ ∧
+    simulation_body iτs iηs (td_env U) (td_expr U) (td_pre U) (td_alloc U) τ (td_post U)
+                    (td_D_pre U) D'.
+
   (** Put together the inner pieces of the interpretation of promises... *)
   Definition promiseN := nroot .@ "promise".
-  Definition int_i_promise_body iτs iηs M N A τ τi γ v :=
-    ∃ U D' M' N',
-      ip_data γ U D' M' N' ∗ ip_impl A τ τi D' M' N' M N v ∗ □ip_sim iτs iηs A τ U D' M'.
-  Definition int_i_promise iτs iηs ξ A τ τi d M N x :=
-    ∃ t γ, ⌜N !! ξ = Some (Task t) ∧ M !! ξ = Some γ ∧ x = Ctid t⌝ ∧
-           inv promiseN (wp_wait t (int_i_promise_body iτs iηs (delete ξ M) (delete ξ N) A τ τi γ)).
+  Definition int_i_promise_body iτs iηs N A τ τi t v :=
+    ∃ U D' N', ip_data t U D' N' ∗ ip_impl A τ τi D' N' N v ∗ □ip_sim iτs iηs A τ U D'.
+  Definition int_i_promise iτs iηs ξ A τ τi d N x :=
+    ∃ t, ⌜N !! ξ = Some (Task t) ∧ x = Ctid t⌝ ∧
+           inv promiseN (wait t (int_i_promise_body iτs iηs N A τ τi)).
 End TypeInterpretation.
 
 Section HeapInterpretation.
-  Context `{WaitPermissions, implStateG Σ, specStateG Σ, wp_axiomaticIrisG _ Σ, taskDataG Σ}.
+  Context `{allG Σ}.
   Implicit Type N : name_map.
-  Implicit Type M : task_map.
   Implicit Type D : conn_map.
   Local Open Scope I.
 
-  Definition int_i_emp D M N: iProp Σ := True.
-  Definition int_s_emp := int_i_emp.
-  Definition int_i_star (iη iη': int_heap) D M N: iProp Σ := iη D M N ∗ iη' D M N.
-  Definition int_s_star := int_i_star.
-  Definition int_i_pt ξ (iτ: int_type) D M N: iProp Σ :=
-    ∃ l d v, ⌜N!!ξ = Some (Loc l) ∧ D!!name ξ = Some d⌝ ∗ mapstoI l v 1%Qp ∗ iτ d M N v.
-  Definition int_s_pt ξ (iτ: int_type) D M N: iProp Σ :=
-    ∃ l d v, ⌜N!!ξ = Some (Loc l) ∧ D!!name ξ = Some d⌝ ∗ mapstoS l v 1%Qp ∗ iτ d M N v.
-  Definition int_i_wait_body γ (η: types.heap) (iη: int_heap) A M N :=
-    ∃ U D' N' M', ip_data γ U D' M' N' ∗ ⌜N ≡[ names η ∖ A]≡ N' ∧ M ≡[names η ∖ A]≡ M'⌝ ∗ iη D' M' N'.
-  Definition int_i_wait ξ A η (iη: int_heap) D M N: iProp Σ :=
-    ∃ t γ, ⌜N!!ξ = Some (Task t) ∧ M!!ξ = Some γ⌝ ∗
-                                               wp_wait t (λ _, int_i_wait_body γ η iη A (delete ξ M)
-                                                                               (delete ξ N)).
+  Definition int_i_emp D N: iProp Σ := True.
+  Definition int_s_emp D N: iProp Σ := True.
+  Definition int_i_star (iη iη': intT_heap) D N: iProp Σ := iη D N ∗ iη' D N.
+  Definition int_s_star (iη iη': intT_heap) D N: iProp Σ := iη D N ∗ iη' D N.
+  Definition int_i_pt ξ (iτ: intT_type) D N: iProp Σ :=
+    ∃ l d v, ⌜N!!ξ = Some (Loc l) ∧ D!!name ξ = Some d⌝ ∗ mapstoI l v 1%Qp ∗ iτ d N v.
+  Definition int_s_pt ξ (iτ: intT_type) D N: iProp Σ :=
+    ∃ l d v, ⌜N!!ξ = Some (Loc l) ∧ D!!name ξ = Some d⌝ ∗ mapstoS l v 1%Qp ∗ iτ d N v.
+  Definition int_i_wait_body (η: hexpr) (iη: intT_heap) A N t (_: val): iProp Σ :=
+    ∃ U D' N', ip_data t U D' N' ∗ ⌜N ≡[ names η ∖ A]≡ N'⌝ ∗ iη D' N'.
+  Definition int_i_wait (ξ: gname) A η (iη: intT_heap) D N: iProp Σ :=
+    ∃ t, ⌜N!!ξ = Some (Task t) ∧ D!!name ξ = Some (VConst (Ctid t))⌝ ∗
+                                                  wait t (int_i_wait_body η iη A N).
+
   (* Use the lower-level interpretations here *)
-  Definition int_s_wait_pre iτs' (iηs': types.heap → int_heap) U σ: iProp Σ :=
-    ∃ N, intΓ iτs' (td_env U) (td_D_pre U) (td_M_pre U) N σ ∗
-              iηs' (td_pre U) (td_D_pre U) (td_M_pre U) N.
-  Definition int_s_wait iτs' iηs' ξ A η D M N :=
-    ∃ t γ U σ,
-      ⌜N!!ξ = Some (Task t) ∧ M!!ξ = Some γ ∧
-      td_post U = η ∧ td_alloc U = A ∧
-      td_M_pre U ≡[names η ∖ A]≡ M⌝ ∧ own γ (to_agree U) ∗
-      t ⤇ run: (subst (of_val <$> σ) (td_expr U)) ∗ int_s_wait_pre iτs' iηs' U σ.
+  Definition int_s_wait_pre iτs' (iηs': hexpr → intT_heap) U N ts σ: iProp Σ :=
+    ∃ Npre N, int_env_pre iτs' (td_env U) (td_D_pre U) Npre σ ∗
+                          iηs' (td_pre U) (td_D_pre U) Npre  ∗
+                          spec_task_agree ts Npre ∗
+                          ⌜Npre ≡[names (td_post U) ∖ td_alloc U]≡ N⌝.
+  
+  Definition int_s_wait iτs' iηs' ξ A η D N: iProp Σ :=
+    ∃ ti ts U σ,
+      ⌜N!!ξ = Some (Task ts) ∧ D!!name ξ = Some (VConst (Ctid ti)) ∧ td_post U = η ∧ td_alloc U = A⌝ ∧
+      task_agree ti U ∗
+      ts ⤇ run: (subst (of_val <$> σ) (td_expr U)) ∗ int_s_wait_pre iτs' iηs' U N ts σ.
+  
 End HeapInterpretation.
 
 Section Interpretations.
-  Context `{WaitPermissions, implStateG Σ, specStateG Σ, wp_axiomaticIrisG _ Σ, taskDataG Σ}.
-  Context `{InitialConfiguration, ∀ t, Proper (pointwise_relation _ (≡) ==> (≡)) (wp_wait t)}.
+  Context `{allG Σ}.
   Implicit Type N: name_map.
-  Implicit Type M: task_map.
   Implicit Type D: conn_map.
   Implicit Type x: val.
   Implicit Type d: val.
   Local Open Scope I.
   
-  Fixpoint int_s_type τ: @int_type Σ :=
+  Fixpoint int_s_type τ: @intT_type Σ :=
     match τ with
     | tbool => int_s_bool
     | tunit => int_s_unit
     | tref ξ => int_s_ref ξ
     | ttask ξ A τ => int_s_promise ξ A τ
     end.
-  Fixpoint int_s_heap_approx iη η: @int_heap Σ :=
+  Fixpoint int_s_heap_approx iη η: @intT_heap Σ :=
     match η with
     | hemp => int_s_emp
     | hstar η η' => int_s_star (int_s_heap_approx iη η) (int_s_heap_approx iη η')
@@ -217,20 +198,20 @@ Section Interpretations.
     end.
   Fixpoint int_s_heap_rec n η :=
     int_s_heap_approx (match n with
-                       | O => λ _ _ _ _, False%I
+                       | O => λ _ _ _, False%I
                        | S n => int_s_heap_rec n
                        end)
                       η.
-  Definition int_s_heap η: @int_heap Σ := λ D M N, ∃ n, int_s_heap_rec n η D M N.
+  Definition int_s_heap η: @intT_heap Σ := λ D N, ∃ n, int_s_heap_rec n η D N.
 
-  Fixpoint int_i_type τ: @int_type Σ :=
+  Fixpoint int_i_type τ: @intT_type Σ :=
     match τ with
     | tbool => int_i_bool
     | tunit => int_i_unit
     | tref ξ => int_i_ref ξ
     | ttask ξ A τ => int_i_promise int_s_type int_s_heap ξ A τ (int_i_type τ)
     end.
-  Fixpoint int_i_heap η: @int_heap Σ :=
+  Fixpoint int_i_heap η: @intT_heap Σ :=
     match η with
     | hemp => int_i_emp
     | hstar η η' => int_i_star (int_i_heap η) (int_i_heap η')
@@ -238,102 +219,119 @@ Section Interpretations.
     | hwait ξ A η => int_i_wait ξ A η (int_i_heap η)
     end.
 
-  Definition int_s_env := intΓ int_s_type.
-  Definition int_i_env := intΓ int_i_type.
+  Definition int_s_env := int_env_pre int_s_type.
+  Definition int_i_env := int_env_pre int_i_type.
   
   (** Basic properties of interpretation *)
-  Global Instance int_s_type_persistent τ d M N v:  PersistentP (int_s_type τ d M N v).
+  Global Instance int_s_type_persistent τ d N v:  PersistentP (int_s_type τ d N v).
   Proof. destruct τ; apply _. Qed.
-  Global Instance int_i_type_persistent τ d M N v:  PersistentP (int_i_type τ d M N v).
+  Global Instance int_i_type_persistent τ d N v:  PersistentP (int_i_type τ d N v).
   Proof. destruct τ; apply _. Qed.
-  Global Instance int_s_env_persistent Γ D M N σ: PersistentP (int_s_env Γ D M N σ).
+  Global Instance int_s_env_persistent Γ D N σ: PersistentP (int_s_env Γ D N σ).
   Proof. apply _. Qed.
-  Global Instance int_i_env_persistent Γ D M N σ: PersistentP (int_i_env Γ D M N σ).
+  Global Instance int_i_env_persistent Γ D N σ: PersistentP (int_i_env Γ D N σ).
   Proof. apply _. Qed.
 
+  Notation ov x := (overlap (names x)).
   Global Instance int_s_type_local τ:
-    Proper ((=) ==> overlap (names τ) ==> overlap (names τ) ==> (=) ==> (⊣⊢)) (int_s_type τ).
+    Proper ((=) ==> ov τ ==> (=) ==> (⊣⊢)) (int_s_type τ).
   Proof.
-    induction τ; intros d ? <- M M' eqM N N' eqN x ? <-; cbn; try done.
+    induction τ; intros d ? <- N N' eqN x ? <-; cbn; try done.
     - rewrite /int_s_ref /int_i_ref.
       rewrite eqN; first done.
       cbn; set_solver.
     - rewrite /int_s_promise.
-      f_equiv; intro γ.
       f_equiv; intro T.
-      do 3 f_equiv; intro t.
-      rewrite (eqM ξ) ?(eqN ξ).
-      2,3: by apply elem_of_union_l, elem_of_singleton.
-      do 3 f_equiv.
+      f_equiv; intro Npre.
+      do 2 f_equiv.
+      rewrite (eqN ξ); last (clear; set_solver).
+      f_equiv.
       apply (overlap_iff (names (ttask ξ A τ))); last done.
       apply union_subseteq_r.
   Qed.
 
-  Global Instance int_i_type_local τ:
-    Proper ((=) ==> overlap (names τ) ==> overlap (names τ) ==> (=) ==> (⊣⊢)) (int_i_type τ).
+  Instance wait_Proper t: Proper (pointwise_relation _ (pointwise_relation _ (≡)) ==> (⊣⊢)) (wait t).
   Proof.
-    induction τ; intros d ? <- M M' eqM N N' eqN x ? <-; cbn; try done.
+    intros ϕ ϕ' eqϕ.
+    rewrite equiv_dist => [n].
+    apply: wait_nonexpansive => [t' v'].
+    rewrite eqϕ //.
+  Qed.
+  
+  Global Instance int_i_type_local τ:
+    Proper ((=) ==> ov τ ==> (=) ==> (⊣⊢)) (int_i_type τ).
+  Proof.
+    induction τ; intros d ? <- N N' eqN x ? <-; cbn; try done.
     - rewrite /int_i_ref eqN; first done.
       cbn; set_solver.
     - rewrite /int_i_promise /int_i_promise_body /ip_impl.
       rewrite (eqN ξ); last set_solver.
-      rewrite (eqM ξ); last set_solver.
-      do 24 f_equiv.
-      all: apply (overlap_iff ((names (ttask ξ A τ)))).
-      1,3: apply union_subseteq_r.
-      all: by apply overlap_delete_proper.
+      f_equiv; intro t.
+      do 3 f_equiv; intros t' v'.
+      f_equiv; intro U.
+      f_equiv; intro D'.
+      f_equiv; intro N''.
+      do 2 f_equiv.
+      f_equiv; intro d'.
+      do 3 f_equiv.
+      apply (overlap_iff ((names (ttask ξ A τ)))); last done.
+      apply union_subseteq_r.
   Qed.
 
-  Lemma names_heap_star η η': (names_heap (η ⊗ η') ≡ names_heap η ∪ names_heap η')%C.
+  Lemma exists_or {A} (P Q: A → Prop): ((∃ x: A, P x ∨ Q x) ↔ (∃ x: A, P x) ∨ (∃ x: A, Q x))%type.
+  Proof. clear H Σ. firstorder. Qed.
+  
+  Lemma conn_heap_star η η': (conn_heap (η ⊗ η') ≡ conn_heap η ∪ conn_heap η')%C.
   Proof.
-    rewrite /names_heap => ξ.
+    rewrite /conn_heap => ξ.
     rewrite elem_of_union !elem_of_of_list !elem_of_list_fmap /=.
     setoid_rewrite elem_of_elements.
     change (names (hstar η η')) with (names η ∪ names η').
     setoid_rewrite elem_of_union.
-    split.
-    - intros [? [? [?|?]]]; eauto.
-    - intros [[? [??]]|[? [??]]]; eauto.
+    rewrite -exists_or.
+    apply exist_proper; intro.
+    tauto.
   Qed.
   
   Lemma int_s_heap_approx_local
-        iη (iη_proper: ∀ (η: types.heap),
-               Proper (overlap (names_heap η) ==> overlap (names η) ==> overlap (names η) ==> (⊣⊢))
-                      (iη η)) η:
-    Proper (overlap (names_heap η) ==> overlap (names η) ==> overlap (names η) ==> (⊣⊢))
-           (int_s_heap_approx iη η).
+        iη (iη_proper: ∀ (η: hexpr),
+               Proper (overlap (conn_heap η) ==> ov η ==> (⊣⊢)) (iη η)) η:
+    Proper (overlap (conn_heap η) ==> ov η ==> (⊣⊢)) (int_s_heap_approx iη η).
   Proof.
-    induction η; intros D D' eqD M M' eqM N N' eqN; cbn.
+    induction η; intros D D' eqD N N' eqN; cbn.
     - done.
     - rewrite /int_s_star /int_i_star.
       f_equiv; [apply IHη1|apply IHη2].
       all: eapply overlap_mono; eauto.
       all: cbn.
-      1,4: rewrite names_heap_star.
-      1,3,4: apply union_subseteq_l.
-      all: apply union_subseteq_r.
+      1,3: rewrite conn_heap_star.
+      all: clear; set_solver.
     - rewrite /int_s_pt.
       setoid_rewrite (eqN ξ); last (rewrite /= elem_of_union elem_of_singleton; auto).
       rewrite eqD; cycle 1.
-      { rewrite elem_of_names_heap.
+      { rewrite elem_of_conn_heap.
         exists ξ; split; auto.
         rewrite /= elem_of_union elem_of_singleton; auto. }
-      enough (∀ d v, int_s_type τ d M N v ⊣⊢ int_s_type τ d M' N' v) as eqint.
+      enough (∀ d v, int_s_type τ d N v ⊣⊢ int_s_type τ d N' v) as eqint.
       { by setoid_rewrite eqint. }
       intros; apply int_s_type_local; auto.
-      all: eapply overlap_mono; eauto.
-      all: intros ??; apply elem_of_union; auto.
+      eapply overlap_sub; last done.
+      apply union_subseteq_r.
     - rewrite /int_s_wait /=.
-      do 10 f_equiv.
-      rewrite (eqN ξ); last set_solver.
-      rewrite (eqM ξ); last set_solver.
-      do 4 f_equiv.
-      all: eapply overlap_iff; last done.
-      all: apply union_subseteq_r.
+      f_equiv; intro ti.
+      f_equiv; intro ts.
+      f_equiv; intro U.
+      f_equiv; intro σ.
+      f_equiv.
+      rewrite (eqN ξ); last (clear; set_solver).
+      rewrite (eqD (name ξ)); first done.
+      rewrite elem_of_conn_heap; exists ξ.
+      split; auto.
+      clear; set_solver.
   Qed.
 
   Lemma int_s_heap_rec_local n: ∀ η,
-      Proper (overlap (names_heap η) ==> overlap (names η) ==> overlap (names η) ==> (⊣⊢))
+      Proper (overlap (conn_heap η) ==> overlap (names η) ==> (⊣⊢))
              (int_s_heap_rec n η).
   Proof.
     induction n as [|n IH]; intros; cbn; apply int_s_heap_approx_local; auto.
@@ -341,64 +339,56 @@ Section Interpretations.
   Qed.
 
   Lemma int_s_heap_local η:
-    Proper (overlap (names_heap η) ==> overlap (names η) ==> overlap (names η) ==> (⊣⊢))
-           (int_s_heap η).
+    Proper (overlap (conn_heap η) ==> overlap (names η) ==> (⊣⊢)) (int_s_heap η).
   Proof.
-    intros D D' M M' eqM eqD N N' eqN.
+    intros D D' eqD N N' eqN.
     rewrite /int_s_heap.
     f_equiv; intro n.
     apply int_s_heap_rec_local; done.
   Qed.
   
   Lemma int_i_heap_local η:
-    Proper (overlap (names_heap η) ==> overlap (names η) ==> overlap (names η) ==> (⊣⊢))
-           (int_i_heap η).
+    Proper (overlap (conn_heap η) ==> overlap (names η) ==> (⊣⊢)) (int_i_heap η).
   Proof.
-    induction η; intros D D' eqD M M' eqM N N' eqN; cbn.
+    induction η; intros D D' eqD N N' eqN; cbn.
     - done.
     - rewrite /int_s_star /int_i_star.
       f_equiv; [apply IHη1|apply IHη2].
-      all: eapply overlap_mono; eauto.
-      all: cbn.
-      1,4: rewrite names_heap_star.
-      1,3,4: apply union_subseteq_l.
-      all: apply union_subseteq_r.
+      all: eapply overlap_sub; last done.
+      1,3: rewrite conn_heap_star.
+      all: clear; set_solver.
     - rewrite /int_i_pt.
       rewrite (eqN ξ); last set_solver.
       rewrite (eqD (name ξ)).
-      2: rewrite elem_of_names_heap /=.
+      2: rewrite elem_of_conn_heap /=.
       2: eexists _; split; auto; apply elem_of_union; rewrite elem_of_singleton; auto.
       assert (N ≡[ names τ ]≡ N') as eqN'.
       { intros ξ' inξ; apply eqN; set_solver. }
-      assert (M ≡[ names τ ]≡ M') as eqM'.
-      { intros ξ' inξ; apply eqM; set_solver. }
-      enough (∀ d v, int_i_type τ d M N v ⊣⊢ int_i_type τ d M' N' v) as eqτ.
+      enough (∀ d v, int_i_type τ d N v ⊣⊢ int_i_type τ d N' v) as eqτ.
       { by setoid_rewrite eqτ. }
       intros; by apply int_i_type_local.
     - rewrite /int_i_wait /int_i_wait_body.
       rewrite (eqN ξ); last set_solver.
-      rewrite (eqM ξ); last set_solver.
-      enough (∀ M'' N'', (delete ξ N ≡[ names η ∖ A ]≡ N'' ∧ delete ξ M ≡[ names η ∖ A ]≡ M'')
-                           ↔ (delete ξ N' ≡[ names η ∖ A ]≡ N'' ∧ delete ξ M' ≡[ names η ∖ A ]≡ M''))
-        as eqMN'.
-      { by setoid_rewrite eqMN'. }
-      intros.
-      rewrite -!(symmetry_iff (overlap (names η ∖ A)) N'').
-      rewrite -!(symmetry_iff (overlap (names η ∖ A)) M'').
-      f_equiv.
-      all: apply (overlap_iff (names (hwait ξ A η))).
-      1,3: apply union_subseteq_r.
-      all: by apply overlap_delete_proper.
+      rewrite (eqD (name ξ)).
+      2: rewrite elem_of_conn_heap; exists ξ; split; auto; clear; set_solver.
+      f_equiv; intro t.
+      do 2 f_equiv.
+      intros t' _.
+      f_equiv; intro U.
+      f_equiv; intro D''.
+      f_equiv; intro N''.
+      do 3 f_equiv.
+      rewrite -!(symmetry_iff (overlap _) N'').
+      eapply overlap_iff; last done.
+      apply union_subseteq_r.
   Qed.
 
-  Lemma intΓ_local (ϕ: type → @int_type Σ)
-        (ϕ_local: ∀ τ, Proper ((=) ==> overlap (names τ) ==> overlap (names τ) ==> (=) ==> (⊣⊢))
-                              (ϕ τ)) Γ:
-    Proper (overlap (names_env Γ) ==> overlap (names Γ) ==> overlap (names Γ) ==> (=) ==> (⊣⊢))
-           (intΓ ϕ Γ).
+  Lemma intΓ_local (ϕ: type → @intT_type Σ)
+        (ϕ_local: ∀ τ, Proper ((=) ==> ov τ ==> (=) ==> (⊣⊢)) (ϕ τ)) Γ:
+    Proper (overlap (conn_env Γ) ==> ov Γ ==> (=) ==> (⊣⊢)) (int_env_pre ϕ Γ).
   Proof.
-    intros D D' eqD M M' eqM N N' eqN σ ? <-.
-    rewrite /intΓ.
+    intros D D' eqD N N' eqN σ ? <-.
+    rewrite /int_env_pre.
     assert (pure_l_and: ∀ P P' (Q Q': iProp Σ) (eqP: (P ↔ P')%type) (eqQ: P → Q ⊣⊢ Q'),
                ⌜P⌝ ∧ Q ⊣⊢ ⌜P'⌝ ∧ Q').
     { intros; rewrite -eqP.
@@ -407,69 +397,71 @@ Section Interpretations.
     { apply and_iff_compat_l, forall_proper; intro.
       destruct (decide (is_Some (Γ!!x))) as [[τ tyx]|]; last tauto.
       rewrite (eqD (var x)); first done.
-      rewrite elem_of_names_env.
+      rewrite elem_of_conn_env.
       exists x; eauto. }
     intros [domσ domD].
     f_equiv; intro x.
     f_equiv; intro τ.
     f_equiv; intro v.
     f_equiv; intro d.
-    destruct (decide (Γ!!x = Some τ)) as [mt|].
-    2: iSplit; iIntros "_ %"; intuition discriminate.
-    assert (var x ∈ names_env Γ) as in_var_x.
-    { rewrite elem_of_names_env; exists x; rewrite mt; eauto. }
-    rewrite (eqD (var x)); last done.
+    rewrite /int_env_data.
+    destruct (decide (Γ !! x = Some τ)) as [type_x|contra].
+    2: iSplit; iIntros "_"; iIntros ([? _]); congruence.
+    rewrite (eqD (var x)).
+    2: rewrite elem_of_conn_env; exists x; rewrite type_x; eauto.
     f_equiv.
-    apply ϕ_local; try done.
-    all: eapply overlap_mono.
-    2,3,4,6,7,8: done.
-    all: intro ξ; rewrite env_elem_of_names; exists x,τ; eauto.
+    apply ϕ_local.
+    1,3: done.
+    apply (overlap_sub (names Γ)); last done.
+    intros ξ inξ.
+    rewrite elem_of_names_env.
+    exists x, τ; auto.
   Qed.
 
   Lemma int_i_env_local Γ: 
-    Proper (overlap (names_env Γ) ==> overlap (names Γ) ==> overlap (names Γ) ==> (=) ==> (⊣⊢))
-           (int_i_env  Γ).
+    Proper (overlap (conn_env Γ) ==> ov Γ ==> (=) ==> (⊣⊢)) (int_i_env  Γ).
   Proof. apply intΓ_local, int_i_type_local. Qed.
   Lemma int_s_env_local Γ: 
-    Proper (overlap (names_env Γ) ==> overlap (names Γ) ==> overlap (names Γ) ==> (=) ==> (⊣⊢))
-           (int_s_env  Γ).
+    Proper (overlap (conn_env Γ) ==> ov Γ ==> (=) ==> (⊣⊢)) (int_s_env  Γ).
   Proof. apply intΓ_local, int_s_type_local. Qed.
-  
-  Lemma int_s_heap_approx_mono ϕ ϕ' (mono: ∀ η D M N, ϕ η D M N -∗ ϕ' η D M N) η:
-    ∀ D M N, int_s_heap_approx ϕ η D M N -∗ int_s_heap_approx ϕ' η D M N.
+
+  Local Open Scope I.
+  Lemma int_s_heap_approx_mono ϕ ϕ' (mono: ∀ η D N, ϕ η D N -∗ ϕ' η D N) η:
+    ∀ D N, int_s_heap_approx ϕ η D N -∗ int_s_heap_approx ϕ' η D N.
   Proof.
     induction η; cbn.
-    - iIntros (???) "$".
-    - iIntros (D M N) "[I1 I2]".
+    - iIntros (??) "$".
+    - iIntros (D N) "[I1 I2]".
       iSplitL "I1".
       + iApply (IHη1 with "I1").
       + iApply (IHη2 with "I2").
-    - iIntros (???) "$".
-    - iIntros (D M N).
+    - iIntros (??) "$".
+    - iIntros (D N).
       rewrite /int_s_wait /int_s_wait_pre.
       iIntros "pre".
       iDestruct "pre" as (t γ U σ) "[names [agree [move pre]]]".
       iExists t,γ,U,σ; iFrame.
       iDestruct "pre" as (N') "wait".
       iExists N'.
-      iDestruct "wait" as "[$ ϕ]".
+      iDestruct "wait" as (N'') "[$ [ϕ rest]]".
+      iExists N''; iFrame.
       iApply (mono with "ϕ").
   Qed.
-  Lemma int_s_heap_rec_S n: ∀ η D M N, int_s_heap_rec n η D M N -∗ int_s_heap_rec (S n) η D M N.
+  Lemma int_s_heap_rec_S n: ∀ η D N, int_s_heap_rec n η D N -∗ int_s_heap_rec (S n) η D N.
   Proof.
     rewrite -Nat.add_1_r.
     induction n as [|n IH]; cbn.
-    all: iIntros (η D M N) "pre"; iApply (int_s_heap_approx_mono with "pre").
-    - iIntros (????) "[]".
+    all: iIntros (η D N) "pre"; iApply (int_s_heap_approx_mono with "pre").
+    - iIntros (???) "[]".
     - exact IH.
   Qed.
   
   Lemma int_s_heap_rec_mono n n' (len: n ≤ n'):
-    ∀ η D M N, int_s_heap_rec n η D M N -∗ int_s_heap_rec n' η D M N.
+    ∀ η D N, int_s_heap_rec n η D N -∗ int_s_heap_rec n' η D N.
   Proof.
     induction len.
-    { iIntros (????) "$". }
-    iIntros (η D M N) "pre".
+    { iIntros (???) "$". }
+    iIntros (η D N) "pre".
     iApply (int_s_heap_rec_S with "[-]").
     iApply (IHlen with "pre").
   Qed.
