theories/closed_meta.v
@@ -1,0 +1,290 @@
+From iris.proofmode Require Import tactics.
+From iris.base_logic.lib Require Import invariants.
+From esop Require Import overlap delayed specification typetranslation types corecalculus.
+From stdpp Require Import gmap coPset.
+
+Section Theory.
+  Context `{allG Σ}.
+  (** Meta theory: The framing lemma *)
+  Definition frame ηf (D D': conn_map): conn_map := D ~[conn_heap ηf]~> D'.
+
+  Lemma frame_generic          
+        (int_ty: type → @intT_type Σ) (int_he: hexpr → @intT_heap Σ) τ (η ηf: hexpr)
+        D D' d v (N N': name_map)
+        (novN: N ≡[names ηf]≡ N')
+        (int_he_split: ∀ D'' N'',
+            int_he (hstar η ηf) D'' N'' ⊣⊢ int_he η D'' N'' ∗ int_he ηf D'' N'')
+        (int_he_local: ∀ η,
+            Proper (overlap (conn_heap η) ==> overlap (names η) ==> (≡)) (int_he η))
+        (disj: names η ⊥ names ηf):
+    int_he ηf D N -∗ (⌜D' !! RET = Some d⌝ ∗ int_ty τ d N' v ∗ int_he η D' N') -∗
+           (⌜frame ηf D D' !! RET = Some d⌝) ∗
+           int_ty τ d N' v ∗ int_he (hstar η ηf) (frame ηf D D') N'.
+  Proof.
+    iIntros "frame [eqd [type heap]]".
+    iFrame.
+    iSplitL "eqd".
+    { iDestruct "eqd" as %eqd.
+      iPureIntro.
+      rewrite /frame lookup_merge_along_not_in //.
+      rewrite elem_of_conn_heap => [[? [? _]]]; done. }
+    rewrite int_he_split.
+    iSplitL "heap".
+    - iApply (int_he_local with "heap").
+      2,3: done.
+      apply overlap_merge_along_r.
+      intro ξ.
+      rewrite !elem_of_conn_heap => [[ξ₁ [eq₁ in₁]] [ξ₂ [eq₂ in₂]]]; subst.
+      injection eq₂ as <-; apply (disj ξ₁); done.
+    - by iApply (int_he_local with "frame"); first apply overlap_merge_along_l.
+  Qed.
+
+  Lemma int_s_rec_split n η η' D N:
+    int_s_heap_rec n (hstar η η') D N ⊣⊢ int_s_heap_rec n η D N ∗ int_s_heap_rec n η' D N.
+  Proof. destruct n; done. Qed.
+  
+  Lemma int_s_heap_split η η' D N:
+    int_s_heap (hstar η η') D N ⊣⊢ (int_s_heap η D N ∗ int_s_heap η' D N).
+  Proof.
+    iSplit.
+    { iIntros "pre".
+      iDestruct "pre" as (n) "pre".
+      rewrite int_s_rec_split.
+      iDestruct "pre" as "[pre pre']".
+      iSplitL "pre"; iExists n; iFrame.
+    } {
+      iIntros "[pre pre']".
+      iDestruct "pre" as (n) "pre".
+      iDestruct "pre'" as (n') "pre'".
+      iExists (max n n').
+      rewrite int_s_rec_split.
+      iSplitL "pre".
+      all: iApply int_s_heap_rec_mono; last iFrame.
+      all: auto with arith.
+    }
+  Qed.
+  
+  Lemma frame_existential Γ e (η: hexpr) A τ (η': hexpr) D D' D'' (ηf: hexpr)
+        (disj': names η' ⊥ names ηf) (disj: names η ⊥ names ηf) (disj'': names ηf ⊥ A):
+    simulation Γ e η A τ η' D D' -∗
+               simulation Γ e (hstar η ηf) A τ (hstar η' ηf) (frame ηf D'' D)
+               (frame ηf D'' D').
+  Proof.
+    iIntros "sim".
+    iIntros (N σ p K) "ctx [env pre] move".
+    rewrite int_s_heap_split.
+    iDestruct "pre" as "[pre frame]".
+    iMod ("sim" with "ctx [env pre] move") as (v) "[post move]".
+    { iSplitL "env".
+      - iApply (int_s_env_local with "env").
+        2-4: done.
+        symmetry.
+        apply overlap_merge_along_r.
+        intro n.
+        rewrite elem_of_conn_heap elem_of_conn_env => [[ξ [??]] [ξ' [eqξ ?]]].
+        subst; discriminate.
+      - iApply (int_s_heap_local with "pre"); last done.
+        rewrite /frame; symmetry.
+        apply: overlap_merge_along_r => [n].
+        rewrite !elem_of_conn_heap => [[ξ [??]] [ξ' [eqξ ?]]]; subst.
+        injection eqξ as <-.
+        apply (disj ξ); done. }
+    iDestruct "post" as (d N') "[eqs [type post]]".
+    iModIntro; iExists v; iFrame.
+    iDestruct "eqs" as %[eqN eqd].
+    iExists d, N'.
+    assert ((of_gset (names ηf): coPset) ⊆ (not_new A: coPset)).
+    { intro x; rewrite elem_of_of_gset elem_of_not_new; exact (disj'' x). }
+    iPoseProof (frame_generic int_s_type int_s_heap τ η' ηf D'' D' d v N N'
+                with "[frame] [$type $post]") as "post".
+    all: try done.
+    { apply overlap_cast, (overlap_sub (not_new A)); last done.
+      intro x; rewrite elem_of_of_gset elem_of_not_new; exact (disj'' x). }
+    - apply int_s_heap_split.
+    - intro; apply int_s_heap_local.
+    - iApply (int_s_heap_local with "frame"); last done.
+      symmetry; apply overlap_merge_along_l.
+    - iDestruct "post" as "[% [$$]]"; auto.
+  Qed.
+
+  Lemma simulation_local Γ e η A τ η':
+    Proper (overlap (conn_env Γ ∪ conn_heap η) ==> overlap ({[RET]} ∪ conn_heap η') ==> (⊣⊢))
+           (simulation Γ e η A τ η').
+  Proof.
+    iIntros (D D' eqD E E' eqE).
+    rewrite /simulation /simulation_body /existential_triple.
+    f_equiv; intro N.
+    f_equiv; intro σ.
+    f_equiv; intro p.
+    f_equiv; intro K.
+    do 2 f_equiv.
+    { f_equiv.
+      - apply int_s_env_local.
+        2-4: done.
+        eapply overlap_sub; last done.
+        apply union_subseteq_l.
+      - apply int_s_heap_local.
+        2,3: done.
+        eapply overlap_sub; last done.
+        apply union_subseteq_r. }
+    do 3 f_equiv; intro v.
+    do 2 f_equiv; intro d.
+    f_equiv; intro N'.
+    f_equiv.
+    { rewrite (eqE RET); first done.
+      clear; set_solver. }
+    f_equiv.
+    apply int_s_heap_local; last done.
+    eapply overlap_sub; last done.
+    apply union_subseteq_r.
+  Qed.
+  
+  Lemma closed_frame Γ e e' (η: hexpr) A τ (η' ηf: hexpr)
+        (disj': names η' ⊥ names ηf) (disj: names η ⊥ names ηf) (disj'': names ηf ⊥ A):
+    delayed_typed Γ η e e' A τ η' -∗
+                  delayed_typed Γ (hstar η ηf) e e' A τ (hstar η' ηf).
+  Proof.
+    iIntros "del".
+    iIntros (D N σ); cbn -[difference].
+    iIntros "[env [pre frame]]".
+    iSpecialize ("del" $! D N σ with "[$env $pre]").
+    iApply (wp_wand with "del").
+    iIntros (v) "post".
+    iDestruct "post" as (N' D' d') "[eqs [type [#sim post]]]".
+    iExists N', (frame ηf D D'), d'.
+    iFrame.
+    iDestruct "eqs" as %[eqN eqD'].
+    iSplit.
+    { iPureIntro; split; auto.
+      rewrite /frame lookup_merge_along_not_in; first done.
+      rewrite elem_of_conn_heap => [[? [? _]]]; done. }
+    iSplit.
+    { iAlways.
+      iIntros (Ns Ds p K) "ctx [env pre] move".
+      rewrite int_s_heap_split.
+      iDestruct "pre" as "[pre frame]".
+      iMod ("sim" with "ctx [$env $pre] move") as (v') "[post move]".
+      iModIntro; iExists v'; iFrame.
+      iDestruct "post" as (d Ns') "[names [type post]]".
+      iDestruct "names" as %[eqNs eqDs].
+      iPoseProof (frame_generic with "frame [type $post]") as "post".
+      - apply overlap_cast, (overlap_sub (not_new A)); last done.
+        intro ξ; rewrite elem_of_of_gset elem_of_not_new; exact (disj'' ξ).
+      - by intros; rewrite int_s_heap_split.
+      - apply int_s_heap_local.
+      - done.
+      - iSplit; first done; iExact "type".
+      - iExists d, _.
+        iDestruct "post" as "[? [$$]]".
+        iDestruct "post" as %->; iPureIntro; auto. }
+    iSplitR "frame"; iApply int_i_heap_local.
+    3,6: iFrame.
+    2: done.
+    - rewrite /frame overlap_merge_along_r; first done.
+      intro n; rewrite !elem_of_conn_heap => [[ξ [??]] [? [eqξ ?]]]; subst.
+      injection eqξ as <-; by apply (disj' ξ).
+    - apply overlap_merge_along_l.
+    - apply overlap_cast, (overlap_sub (not_new A)); last done.
+      intro ξ; rewrite !elem_of_of_gset elem_of_not_new; exact (disj'' ξ).
+  Qed.
+  
+  (** Meta-theory: Strengthening the environment. *)
+  Definition restrict_subst' {A} (e: option A) (τ: option type) :=
+    match τ with Some _ => e | None => None end.
+  Definition restrict_subst {A} (Γ: env) (σ: gmap string A) := merge restrict_subst' σ Γ.
+  Instance: ∀ A, DiagNone (@restrict_subst' A).
+  Proof. done. Qed.
+  Lemma lookup_restrict_subst_is_Some {A} (Γ: env) (σ: gmap string A) x:
+    is_Some (restrict_subst Γ σ !! x) ↔ is_Some (Γ!!x) ∧ is_Some (σ!!x).
+  Proof.
+    rewrite /restrict_subst lookup_merge.
+    enough (∀ o, is_Some (restrict_subst' (σ!!x) o) ↔ is_Some o ∧ is_Some (σ !! x))
+      as -> by done.
+    intros [τ|]; cbn.
+    - intuition eauto.
+    - rewrite -!not_eq_None_Some; tauto.
+  Qed.
+  
+  Lemma restrict_env (int_ty: type → @intT_type Σ) Γ Γ' D N σ (sub: Γ ⊆ Γ'):
+    int_env_pre int_ty Γ' D N σ -∗ int_env_pre int_ty Γ D N (restrict_subst Γ σ).
+  Proof.
+    rewrite /int_env_pre.
+    iIntros "[maps env]".
+    iDestruct "maps" as %[domσ domD].
+    iSplit.
+    { iPureIntro; split; intro.
+      - rewrite lookup_restrict_subst_is_Some.
+        split; last tauto.
+        intro inx; split; auto.
+        eapply domσ, lookup_weaken_is_Some; done.
+      - intro inx.
+        eapply domD, lookup_weaken_is_Some; done. }
+    iIntros (x τ v d) "pre".
+    iDestruct "pre" as %[eqτ [eqv eqd]].
+    iApply ("env" $! x τ v d).
+    iPureIntro.
+    repeat split; auto.
+    - by eapply lookup_weaken.
+    - by rewrite /restrict_subst lookup_merge eqτ in eqv.
+  Qed.
+
+  Lemma subst_restrict_with_type `(ty: typing U Γ e η A τ η'):
+    ∀ σ, subst (restrict_subst Γ σ) e = subst σ e.
+  Proof.
+    induction ty; intros; cbn.
+    1,2,3,6,7,8,9: congruence.
+    - by rewrite /restrict_subst lookup_merge Γx.
+    - rewrite IHty1; do 2 f_equal.
+      rewrite -(IHty2 (delete' x σ)); f_equal.
+      apply map_eq; intro y.
+      rewrite lookup_delete'_cases /restrict_subst !lookup_merge lookup_delete'_cases.
+      destruct (bool_decide_reflect (BNamed y ≠ x)) as [neqx|<-%dec_stable].
+      + rewrite /restrict_subst' /insert'.
+        destruct x; first done.
+        rewrite lookup_insert_ne; congruence.
+      + by destruct (insert' (BNamed y) τ₁ Γ !! y).
+  Qed.
+
+  Lemma restrict_env_fmap `(f: A → B) Γ m:
+    f <$> restrict_subst Γ m = restrict_subst Γ (f <$> m).
+  Proof.
+    apply map_eq; intro y.
+    rewrite /restrict_subst lookup_fmap !lookup_merge lookup_fmap /restrict_subst'.
+    match goal with |- f <$> match ?a with _ => _ end = _ => by destruct a end.
+  Qed.
+  
+  Lemma closed_strengthen U Γ Γ' e e' η A A' τ η'
+        (ty: typing U Γ e η A τ η')
+        (ty': typing U Γ e' η A τ η')
+        (subΓ: Γ ⊆ Γ') (subA: A ⊆ A'):
+    delayed_typed Γ η e e' A τ η' -∗ delayed_typed Γ' η e e' A' τ η'.
+  Proof.
+    assert (not_new A' ⊆ not_new A).
+    { intro; rewrite /not_new !elem_of_difference !elem_of_of_gset.
+      clear -subA; set_solver. }
+    iIntros "spec".
+    iIntros (D N σ) "[env pre]".
+    iSpecialize ("spec" $! D N (restrict_subst Γ σ) with "[env $pre]").
+    { by iApply (restrict_env with "env"). }
+    rewrite restrict_env_fmap (subst_restrict_with_type ty).
+    iApply (wp_wand with "spec").
+    iIntros (v) "post".
+    iDestruct "post" as (N' D' d') "[eqs [type [#sim post]]]".
+    iExists N', D', d'; iFrame.
+    iDestruct "eqs" as %[eqN eqd].
+    iSplit.
+    { iPureIntro; repeat split; auto.        
+      all: eapply overlap_mono; done. }
+    clear eqN N N' σ v; iAlways.
+    iIntros (N σ p K) "ctx [env pre] move".
+    rewrite -(subst_restrict_with_type ty') -restrict_env_fmap.
+    iMod ("sim" $! N (restrict_subst Γ σ) p K with "ctx [env $pre] move") as (v) "[post move]".
+    { by iApply (restrict_env with "env"). }
+    iModIntro; iExists v; iFrame.
+    iDestruct "post" as (d N') "[eqs [type post]]".
+    iExists d, N'; iFrame.
+    iDestruct "eqs" as %[eqN eqD].
+    iPureIntro; repeat split; auto.
+    all: by eapply overlap_mono.
+  Qed.
+End Theory.
